src/high/locations.v
@@ -11,17 +11,17 @@ From iris.proofmode Require Import reduction monpred tactics.
 From iris_named_props Require Import named_props.
 
 From self Require Import extra ipm_tactics solve_view_le.
-From self.algebra Require Import ghost_map ghost_map_map.
-From self.base Require Import primitive_laws post_crash_modality.
+From self.base Require Import primitive_laws.
 From self.lang Require Import lang.
 From self.high Require Import increasing_map monpred_simpl.
-From self.high Require Import dprop dprop_liftings abstract_state lifted_modalities if_rec or_lost.
-From self.high Require Export abstract_state resources protocol modalities post_crash_modality.
+From self.high Require Import dprop generational_resources wrappers protocol.
+From self.high.lib Require Import abstract_state.
+From self.high Require Export modalities.
 From self.high.resources Require Export bumpers preorders auth_map_map abstract_history.
-From self.high.modalities Require Export no_buffer no_flush.
+From self.high.modalities Require Export no_buffer no_flush if_rec or_lost nextgen nextgen_flush.
 
 Section points_to_at.
-  Context `{nvmG Σ, AbstractState ST}.
+  Context `{nvmHighG, AbstractState ST}.
 
   Implicit Types (ℓ : loc) (s : ST) (ss : list ST) (prot : LocationProtocol ST).
 
@@ -41,36 +41,27 @@ Section points_to_at.
       "%lastEq" ∷ ⌜ last ss = Some s ⌝ ∗
       "#locationProtocol" ∷ know_protocol ℓ prot ∗
       "%incrMap" ∷ ⌜ increasing_map (⊑@{ST}) abs_hist ⌝ ∗
-      "#isNaLoc" ∷ is_na_loc ℓ ∗
+      "#isNaLoc" ∷ ⎡ is_na_loc ℓ ⎤ ∗
 
       (* [tHi] is the last message and it agrees with the last state in ss. *)
       "%lookupV" ∷ ⌜ abs_hist !! tHi = Some s ⌝ ∗
       "%nolater" ∷ ⌜ map_no_later abs_hist tHi ⌝ ∗
 
       (* Ownership over the full abstract history. *)
-      "hist" ∷ know_full_history_loc_d ℓ q abs_hist ∗
-      "#histFrag" ∷ know_frag_history_loc_d ℓ tHi s ∗
+      "hist" ∷ ⎡ know_full_history_loc ℓ q abs_hist ⎤ ∗
+      "#histFrag" ∷ ⎡ know_frag_history_loc ℓ tHi s ⎤ ∗
       (* "#offset" ∷ ⎡ ℓ ↪[offset_name]□ offset ⎤ ∗ *)
-      "#offset" ∷ offset_loc ℓ offset ∗
+      "#offset" ∷ ⎡ offset_loc ℓ offset ⎤ ∗
 
-      "knowSV" ∷ know_na_view ℓ q SV ∗
+      "knowSV" ∷ ⎡ know_na_view ℓ q SV ⎤ ∗
       "%slice" ∷ ⌜ map_sequence abs_hist tLo tHi ss ⌝ ∗
-      "#physMsg" ∷ with_gnames (λ nD, ⎡ auth_map_map_frag_singleton phys_history_name ℓ tHi msg ⎤) ∗
+      "#physMsg" ∷ ⎡ know_phys_hist_msg ℓ tHi msg ⎤ ∗
       "#inThreadView" ∷ have_thread_view (SV, msg_persisted_after_view msg, ∅) ∗
       (* We have the [tHi] timestamp in our store view. *)
       "%offsetLe" ∷ ⌜ offset ≤ tHi ⌝ ∗
       "%haveTStore" ∷ ⌜ tHi - offset ≤ SV !!0 ℓ ⌝ ∗
-      "#pers" ∷ (persisted_loc_d ℓ (tLo - offset) ∨ ⌜ tLo - offset = 0 ⌝)
+      "#pers" ∷ (⎡ persisted_loc ℓ (tLo - offset) ⎤ ∨ ⌜ tLo - offset = 0 ⌝)
     )%I.
-
-  Global Instance fractional ℓ (abs_hist : gmap nat ST) :
-    Fractional (λ q, know_full_history_loc_d ℓ q abs_hist).
-  Proof. apply _. Qed.
-
-  Global Instance fractional_2 ℓ (abs_hist : gmap nat ST) q :
-    AsFractional (know_full_history_loc_d ℓ q abs_hist)
-      (λ q, know_full_history_loc_d ℓ q abs_hist) q.
-  Proof. apply _. Qed.
 
   Global Instance mapsto_na_fractional ℓ prot ss :
     Fractional (λ q, mapsto_na ℓ prot q ss).
@@ -81,21 +72,21 @@ Section points_to_at.
     - iNamed 1.
       iDestruct "hist" as "[histP histQ]".
       iDestruct "knowSV" as "[knowSVP knowSVQ]".
-        iSplitL "histP knowSVP".
-        + repeat iExists _. iFrame "#∗%".
-        + repeat iExists _.
-          iFrame "#∗%".
+      iSplitL "histP knowSVP".
+      + repeat iExists _. iFrame "∗#%".
+      + repeat iExists _. iFrame "∗#%".
     - iDestruct 1 as "[L R]".
       iNamed "L".
-      iDestruct "R" as (???????) "(_ & _ & ? & _ & _ & _ & histQ & _ & _ & SV & HIP & ?)".
-      iDestruct (know_full_history_loc_d_agree with "hist histQ") as %->.
-      iDestruct (know_na_view_agree with "knowSV SV") as %->.
+      iDestruct "R" as (???????) "(% & _ & % & #? & % & % & histQ & #? & #? & SV & HIP & ?)".
+      iDestruct (know_full_history_loc_agree with "hist histQ") as %<-.
+      iDestruct (know_na_view_agree with "knowSV SV") as %<-.
+      simplify_map_eq.
       repeat iExists _.
       iFrameF (lastEq).
       iFrameF "locationProtocol".
       iFrameF (incrMap).
       iFrameF "isNaLoc".
-      iFrame "#∗%".
+      iFrame "∗#%".
       iCombine "hist histQ" as "$".
       iCombine "knowSV SV" as "$".
   Qed.
@@ -105,8 +96,8 @@ Section points_to_at.
   Proof. split; [done | apply _]. Qed.
 
   Program Definition have_msg_after_fence msg : dProp Σ :=
-    MonPred (λ i,
-      ⌜ msg.(msg_store_view) ⊑ (store_view i.1) ⌝
+    MonPred (λ TV,
+      ⌜ msg.(msg_store_view) ⊑ (store_view TV) ⌝
       (* ∗ *)
       (* ⌜ msg.(msg_persisted_after_view) ⊑ (flush_view i.1 ⊔ buffer_view i.1) ⌝ *)
     )%I _.
@@ -136,11 +127,11 @@ Section points_to_at.
       "%slicePhys" ∷ ⌜ map_sequence phys_hist tLo tS ms ⌝ ∗
       "%nolater" ∷ ⌜ map_no_later abs_hist tS ⌝ ∗
       "%absPhysHistDomEq" ∷ ⌜ dom abs_hist = dom phys_hist ⌝ ∗
-      "#isAtLoc" ∷ is_at_loc ℓ ∗
+      "#isAtLoc" ∷ ⎡ is_at_loc ℓ ⎤ ∗
       "#locationProtocol" ∷ know_protocol ℓ prot ∗
       "%incrMap" ∷ ⌜ increasing_map (⊑@{ST}) abs_hist ⌝ ∗
       "#absHist" ∷
-        ([∗ map] t ↦ s ∈ abs_hist, know_frag_history_loc_d ℓ t s) ∗
+        ([∗ map] t ↦ s ∈ abs_hist, ⎡ know_frag_history_loc ℓ t s ⎤) ∗
       "#physHist" ∷
         ([∗ map] t ↦ msg ∈ phys_hist,
           (* When we load a message for this location only the views in that
@@ -150,8 +141,8 @@ Section points_to_at.
           requirement to make [mapsto_at] flush free due to how predicates are
           used in [wp_load_at] (only objective things can be extracted). *)
           have_msg_after_fence msg ∗
-          lift_d (λ nD, auth_map_map_frag_singleton phys_history_name ℓ t msg)) ∗
-      "#offset" ∷ offset_loc ℓ offset ∗
+          ⎡ know_phys_hist_msg ℓ t msg ⎤) ∗
+      "#offset" ∷ ⎡ offset_loc ℓ offset ⎤ ∗
       "#tSLe" ∷ have_SV ℓ (tS - offset)).
 
 End points_to_at.
@@ -172,7 +163,9 @@ Notation "l ↦_{ prot }^{ q } ss" := (mapsto_na l prot q ss) (at level 20).
 Notation "l ↦_AT^{ prot } ss" := (mapsto_at l prot ss) (at level 20).
 
 Section mapsto_at_lemmas.
-  Context `{nvmG Σ, AbstractState ST}.
+  Context `{nvmHighG, AbstractState ST}.
+
+  Set Default Proof Using "Type*".
 
   Implicit Types (ℓ : loc) (s : ST) (ss : list ST) (prot : LocationProtocol ST).
 
@@ -202,8 +195,8 @@ Section mapsto_at_lemmas.
 
   Definition lb_base ℓ prot offset tS (s : ST) : dProp Σ :=
     "#locationProtocol" ∷ know_protocol ℓ prot ∗
-    "#knowFragHist" ∷ know_frag_history_loc_d ℓ tS s ∗
-    "#offset" ∷ offset_loc ℓ offset ∗
+    "#knowFragHist" ∷ ⎡ know_frag_history_loc ℓ tS s ⎤ ∗
+    "#offset" ∷ ⎡ offset_loc ℓ offset ⎤ ∗
     "#tSLe" ∷ have_SV ℓ (tS - offset).
 
   Definition store_lb ℓ prot (s : ST) : dProp Σ :=
@@ -217,20 +210,20 @@ Section mapsto_at_lemmas.
       persisted. The later case is for after a crash where we don't have
       anything in the flush view. *)
       "viewFact" ∷ (have_FV_strong ℓ (tF - offset) ∨
-                    persisted_loc_d ℓ (tF - offset))%I.
+                    ⎡ persisted_loc ℓ (tF - offset) ⎤).
 
   Program Definition persist_lb ℓ prot (sP : ST) : dProp Σ :=
     ∃ tP offset,
       "#lbBase" ∷ lb_base ℓ prot offset tP sP ∗
       (* We have the persisted state in our store view. *)
       "#tPLe" ∷ have_FV ℓ (tP - offset) ∗
-      "persisted" ∷ persisted_loc_d ℓ (tP - offset).
+      "persisted" ∷ ⎡ persisted_loc ℓ (tP - offset) ⎤.
 
   Definition crashed_in prot ℓ s : dProp Σ :=
     ∃ CV,
       "#persistLb" ∷ persist_lb ℓ prot (prot.(p_bumper) s) ∗
-      "#crashed" ∷ crashed_at_d CV ∗
-      "#crashedIn" ∷ crashed_in_mapsto_d ℓ s ∗
+      "#crashed" ∷ ⎡ crashed_at CV ⎤ ∗
+      "#crashedIn" ∷ ⎡ crashed_in ℓ s ⎤ ∗
       "%inCV" ∷ ⌜ ℓ ∈ dom CV ⌝.
 
   Global Instance crashed_in_persistent prot ℓ s :
@@ -240,7 +233,7 @@ Section mapsto_at_lemmas.
   (* [ℓ] was not recovered at the last crash. *)
   Definition lost ℓ : dProp Σ :=
     ∃ CV,
-      "#crashed" ∷ crashed_at_d CV ∗
+      "#crashed" ∷ ⎡ crashed_at CV ⎤ ∗
       "%notInCV" ∷ ⌜ℓ ∉ dom CV⌝.
 
   Lemma store_lb_protocol ℓ prot s :
@@ -295,26 +288,24 @@ Section mapsto_at_lemmas.
 
   (* Lemmas for [crashed_in]. *)
 
-  Lemma crashed_in_mapsto_d_agree `{Countable ST} ℓ (s1 s2 : ST) :
-    crashed_in_mapsto_d ℓ s1 -∗ crashed_in_mapsto_d ℓ s2 -∗ ⌜ s1 = s2 ⌝.
+  Lemma base_crashed_in_agree `{Countable ST} ℓ (s1 s2 : ST) :
+    wrappers.crashed_in ℓ s1 -∗ wrappers.crashed_in ℓ s2 -∗ ⌜ s1 = s2 ⌝.
   Proof.
-    iModel.
     simpl.
+    rewrite /wrappers.crashed_in.
     iDestruct 1 as (? eq1) "pts1".
-    simpl.
-    monPred_simpl.
-    iIntros ([??] [? [= <-]]).
-    simpl. iDestruct 1 as (? e2) "pts2".
+    iDestruct 1 as (? eq2) "pts2".
     iDestruct (ghost_map_elem_agree with "pts1 pts2") as %->.
     iPureIntro.
     congruence.
   Qed.
 
   Lemma crashed_in_agree prot ℓ s s' :
-    crashed_in prot ℓ s -∗ crashed_in prot ℓ s' -∗ ⌜ s = s' ⌝. Proof.
+    crashed_in prot ℓ s -∗ crashed_in prot ℓ s' -∗ ⌜ s = s' ⌝.
+  Proof.
     iNamed 1.
     iDestruct 1 as (?) "(? & ? & ? & ?)".
-    iDestruct (crashed_in_mapsto_d_agree with "crashedIn [$]") as %->.
+    iDestruct (base_crashed_in_agree with "crashedIn [$]") as %->.
     done.
   Qed.
 
@@ -330,7 +321,7 @@ Section mapsto_at_lemmas.
     crashed_in prot ℓ s -∗ if_rec ℓ P -∗ P.
   Proof.
     iNamed 1. iNamed "persistLb". iIntros "P".
-    iDestruct (persisted_loc_d_weak with "persisted") as "persisted2".
+    iDestruct (persisted_loc_weak with "persisted") as "persisted2".
     { apply le_0_n. }
     iApply "P"; iFrame "#%".
     iPureIntro. apply elem_of_dom. done.
@@ -443,7 +434,7 @@ Section mapsto_at_lemmas.
     iFrameF (slice). iFrame "physMsg". iFrame "inThreadView".
     iSplitPure; first done.
     iFrameF (haveTStore).
-    iLeft. iApply persisted_loc_d_weak; last done. lia.
+    iLeft. iApply persisted_loc_weak; last done. lia.
   Qed.
 
   Lemma mapsto_na_persist_lb_last ℓ prot q ss s `{!AntiSymm (=) (⊑@{ST})} :
@@ -510,48 +501,50 @@ Section mapsto_at_lemmas.
     BufferFree (mapsto_na ℓ prot q ss).
   Proof. apply _. Qed.
 
-  Lemma post_crash_persist_lb (ℓ : loc) prot (s : ST) :
-    persist_lb ℓ prot s ⊢
-    <PC>
-      persist_lb ℓ prot (prot.(p_bumper) s) ∗
-      ∃ s', ⌜ s ⊑ s' ⌝ ∗ crashed_in prot ℓ s'.
-  Proof.
-    iNamed 1. iNamed "lbBase".
-    rewrite /know_protocol.
-    iNamed "locationProtocol".
-    iDestruct (post_crash_frag_history with "knowPreorder offset knowBumper knowFragHist") as "H".
-    iCrashIntro.
-    iDestruct "persisted" as "(#persisted & (% & %tC & [% %] & #crashed))".
-    iApply (if_rec_get with "crashed persisted"); first done.
-    iModIntro.
-    iDestruct "offset" as (???) "[crashed' offset]".
-    iDestruct (crashed_at_d_agree with "crashed crashed'") as %<-.
-    iClear "crashed'".
-    simplify_eq.
-    iDestruct "H" as (sC ????) "(#crashed' & ? & #hist & ? & impl)".
-    iDestruct (crashed_at_d_agree with "crashed crashed'") as %<-.
-    iClear "crashed'".
-    assert (tC = tC0) as <- by congruence.
-    iDestruct ("impl" with "[%]") as "[% ?]"; first lia.
-    iSplit.
-    * iExists _, _.
-      iFrame "∗#".
-      assert (tP - (offset + tC) = 0) as -> by lia.
-      iFrame "persisted".
-      iDestruct (have_SV_0) as "$".
-      iDestruct (have_FV_0) as "$".
-    * iExists sC. iSplitPure; first done.
-      iExists _. iFrame "crashed". iFrame.
-      iSplit; last (iPureIntro; apply elem_of_dom; done).
-      iExists (offset + tC), (offset + tC).
-      assert ((offset + tC - (offset + tC)) = 0) as -> by lia.
-      iFrame "#∗".
-      iDestruct (have_SV_0) as "$".
-      iDestruct (have_FV_0) as "$".
-  Qed.
+  (* TODO: restore this lemma *)
+  (* Lemma nextgen_persist_lb (ℓ : loc) prot (s : ST) : *)
+  (*   persist_lb ℓ prot s ⊢ *)
+  (*   <NG> *)
+  (*     (persist_lb ℓ prot (prot.(p_bumper) s) ∗ *)
+  (*      ∃ s', ⌜ s ⊑ s' ⌝ ∗ crashed_in prot ℓ s'). *)
+  (* Proof. *)
+  (*   iNamed 1. iNamed "lbBase". *)
+  (*   iModIntro. *)
+  (*   iDestruct "persisted" as "(persisted & %CV & % & crashed_at)". *)
+  (*   iDestruct (post_crash_frag_history with "knowPreorder offset knowBumper knowFragHist") as "H". *)
+  (*   iCrashIntro. *)
+  (*   iDestruct "persisted" as "(#persisted & (% & %tC & [% %] & #crashed))". *)
+  (*   iApply (if_rec_get with "crashed persisted"); first done. *)
+  (*   iModIntro. *)
+  (*   iDestruct "offset" as (???) "[crashed' offset]". *)
+  (*   iDestruct (crashed_at_d_agree with "crashed crashed'") as %<-. *)
+  (*   iClear "crashed'". *)
+  (*   simplify_eq. *)
+  (*   iDestruct "H" as (sC ????) "(#crashed' & ? & #hist & ? & impl)". *)
+  (*   iDestruct (crashed_at_d_agree with "crashed crashed'") as %<-. *)
+  (*   iClear "crashed'". *)
+  (*   assert (tC = tC0) as <- by congruence. *)
+  (*   iDestruct ("impl" with "[%]") as "[% ?]"; first lia. *)
+  (*   iSplit. *)
+  (*   * iExists _, _. *)
+  (*     iFrame "∗#". *)
+  (*     assert (tP - (offset + tC) = 0) as -> by lia. *)
+  (*     iFrame "persisted". *)
+  (*     iDestruct (have_SV_0) as "$". *)
+  (*     iDestruct (have_FV_0) as "$". *)
+  (*   * iExists sC. iSplitPure; first done. *)
+  (*     iExists _. iFrame "crashed". iFrame. *)
+  (*     iSplit; last (iPureIntro; apply elem_of_dom; done). *)
+  (*     iExists (offset + tC), (offset + tC). *)
+  (*     assert ((offset + tC - (offset + tC)) = 0) as -> by lia. *)
+  (*     iFrame "#∗". *)
+  (*     iDestruct (have_SV_0) as "$". *)
+  (*     iDestruct (have_FV_0) as "$". *)
+  (* Qed. *)
 
-  Global Instance persist_lb_into_crash ℓ prot s : IntoCrash _ _ :=
-    post_crash_persist_lb ℓ prot s.
+  (* TODO: restore this lemma *)
+  (* Global Instance persist_lb_into_crash ℓ prot s : IntoCrash _ _ := *)
+  (*   post_crash_persist_lb ℓ prot s. *)
 
   (* This lemma is commented out as it doesn't seem useful. *)
   (* Lemma post_crash_flush_lb (ℓ : loc) prot (s : ST) : *)
@@ -575,28 +568,29 @@ Section mapsto_at_lemmas.
   (* Global Instance flush_lb_into_crash ℓ prot s : IntoCrash _ _ := *)
   (*   post_crash_flush_lb ℓ prot s. *)
 
-  Lemma post_crash_store_lb (ℓ : loc) prot (s : ST) :
-    store_lb ℓ prot s -∗
-    <PC> if_rec ℓ (∃ (s' : ST), persist_lb ℓ prot s').
-  Proof.
-    iNamed 1. iNamed "lbBase".
-    iNamed "locationProtocol".
-    iDestruct (post_crash_frag_history
-      with "knowPreorder offset knowBumper knowFragHist") as "#H".
-    iCrashIntro.
-    iDestruct (if_rec_is_persisted ℓ) as "pers".
-    iModIntro.
-    iDestruct "H" as (sC ????) "(#crashed & ? & ? & ? & impl)".
-    iDestruct "offset" as (???) "(crashed' & ?)".
-    iDestruct (crashed_at_d_agree with "crashed crashed'") as %->.
-    simplify_eq.
-    iExistsN.
-    iFrame.
-    replace (offset + tC - (offset + tC)) with 0 by lia.
-    iDestruct (have_SV_0) as "$".
-    iDestruct (have_FV_0) as "$".
-    iFrame "pers".
-  Qed.
+  (* TODO: restore this lemma *)
+  (* Lemma post_crash_store_lb (ℓ : loc) prot (s : ST) : *)
+  (*   store_lb ℓ prot s -∗ *)
+  (*   <PC> if_rec ℓ (∃ (s' : ST), persist_lb ℓ prot s'). *)
+  (* Proof. *)
+  (*   iNamed 1. iNamed "lbBase". *)
+  (*   iNamed "locationProtocol". *)
+  (*   iDestruct (post_crash_frag_history *)
+  (*     with "knowPreorder offset knowBumper knowFragHist") as "#H". *)
+  (*   iCrashIntro. *)
+  (*   iDestruct (if_rec_is_persisted ℓ) as "pers". *)
+  (*   iModIntro. *)
+  (*   iDestruct "H" as (sC ????) "(#crashed & ? & ? & ? & impl)". *)
+  (*   iDestruct "offset" as (???) "(crashed' & ?)". *)
+  (*   iDestruct (crashed_at_d_agree with "crashed crashed'") as %->. *)
+  (*   simplify_eq. *)
+  (*   iExistsN. *)
+  (*   iFrame. *)
+  (*   replace (offset + tC - (offset + tC)) with 0 by lia. *)
+  (*   iDestruct (have_SV_0) as "$". *)
+  (*   iDestruct (have_FV_0) as "$". *)
+  (*   iFrame "pers". *)
+  (* Qed. *)
 
   (* Global Instance store_lb_into_crash ℓ prot s : IntoCrash _ _ := *)
   (*   post_crash_store_lb ℓ prot s. *)
@@ -608,159 +602,159 @@ Section mapsto_at_lemmas.
   (*   map_sequence abs_hist tLo t ss. *)
   (* Proof. *)
 
-  Lemma post_crash_mapsto_na ℓ prot `{!ProtocolConditions prot} q (ss : list ST) :
-    ℓ ↦_{prot}^{q} ss ⊢
-    <PC>
-      if_rec ℓ (∃ ss' s,
-        ⌜ (ss' ++ [s]) `prefix_of` ss ⌝ ∗
-        crashed_in prot ℓ s ∗
-        ℓ ↦_{prot}^{q} ((p_bumper prot <$> ss') ++ [prot.(p_bumper) s])).
-  Proof.
-    rewrite /mapsto_na.
-    iNamed 1.
-    iNamed "locationProtocol".
-    iDestruct (post_crash_know_full_history_loc with "[$knowBumper $hist]") as "H".
-    iCrashIntro.
-    iDestruct (if_rec_is_persisted ℓ) as "persisted".
-    iModIntro.
-    iDestruct "offset" as (tC CV cvLook) "(crashed & offset)".
-    iDestruct "H" as (? s2 v absHistLook)
-      "(bumper & #crashedIn & offset' & fullHist & fragHist & #phys)".
-    iDestruct (offset_loc_agree with "offset offset'") as %<-.
-    iClear "offset'".
-    assert (offset + tC ≤ tHi). { eapply map_no_later_Some; done. }
+  (* TODO: restore this lemma *)
+  (* Lemma post_crash_mapsto_na ℓ prot `{!ProtocolConditions prot} q (ss : list ST) : *)
+  (*   ℓ ↦_{prot}^{q} ss ⊢ *)
+  (*   <PC> *)
+  (*     if_rec ℓ (∃ ss' s, *)
+  (*       ⌜ (ss' ++ [s]) `prefix_of` ss ⌝ ∗ *)
+  (*       crashed_in prot ℓ s ∗ *)
+  (*       ℓ ↦_{prot}^{q} ((p_bumper prot <$> ss') ++ [prot.(p_bumper) s])). *)
+  (* Proof. *)
+  (*   rewrite /mapsto_na. *)
+  (*   iNamed 1. *)
+  (*   iNamed "locationProtocol". *)
+  (*   iDestruct (post_crash_know_full_history_loc with "[$knowBumper $hist]") as "H". *)
+  (*   iCrashIntro. *)
+  (*   iDestruct (if_rec_is_persisted ℓ) as "persisted". *)
+  (*   iModIntro. *)
+  (*   iDestruct "offset" as (tC CV cvLook) "(crashed & offset)". *)
+  (*   iDestruct "H" as (? s2 v absHistLook) *)
+  (*     "(bumper & #crashedIn & offset' & fullHist & fragHist & #phys)". *)
+  (*   iDestruct (offset_loc_agree with "offset offset'") as %<-. *)
+  (*   iClear "offset'". *)
+  (*   assert (offset + tC ≤ tHi). { eapply map_no_later_Some; done. } *)
 
-    iAssert (⌜ tLo ≤ offset + tC ⌝)%I as %?.
-    { iDestruct "pers" as "[(_ & (%CV' & % & [% %] & crashed'))|%eq]".
-      - iDestruct (crashed_at_d_agree with "crashed crashed'") as %<-.
-        simplify_eq. iPureIntro. lia.
-      - iPureIntro. lia. }
-    eassert _ as HT. { eapply map_sequence_prefix_alt; done. }
-    destruct HT as (ss' & prefix & slice').
+  (*   iAssert (⌜ tLo ≤ offset + tC ⌝)%I as %?. *)
+  (*   { iDestruct "pers" as "[(_ & (%CV' & % & [% %] & crashed'))|%eq]". *)
+  (*     - iDestruct (crashed_at_d_agree with "crashed crashed'") as %<-. *)
+  (*       simplify_eq. iPureIntro. lia. *)
+  (*     - iPureIntro. lia. } *)
+  (*   eassert _ as HT. { eapply map_sequence_prefix_alt; done. } *)
+  (*   destruct HT as (ss' & prefix & slice'). *)
 
-    iExists ss', s2.
-    iSplitPure; first done.
-    iSplit.
-    { rewrite /crashed_in.
-      iExists CV.
-      iFrame "crashed crashedIn".
-      iSplit; last (iPureIntro; apply elem_of_dom; done).
-      iFrame.
-      iExists (offset + tC), (offset + tC).
-      assert ((offset + tC - (offset + tC)) = 0) as -> by lia.
-      iFrame "persisted".
-      iFrame "#∗".
-      iDestruct (have_SV_0) as "$".
-      iDestruct (have_FV_0) as "$". }
-    iExists tLo, (offset + tC), (offset + tC), ∅, _, (Msg _ ∅ ∅ ∅), _.
-    iFrame. iFrame "#".
-    iSplitPure. { apply last_snoc. }
-    iSplitPure.
-    { apply: increasing_map_fmap.
-      apply increasing_map_filter.
-      done. }
-    iSplitPure.
-    { rewrite lookup_fmap.
-      rewrite drop_above_lookup_t.
-      rewrite absHistLook.
-      done. }
-    iSplitPure. {
-      apply map_no_later_fmap.
-      apply map_no_later_drop_above. }
-    iSplitPure.
-    { rewrite -fmap_snoc.
-      apply map_sequence_fmap.
-      apply map_sequence_drop_above.
-      done. }
-    iSplit. { simpl. iApply monPred_in_bottom. }
-    iSplitPure; first lia.
-    iSplitPure; first lia.
-    iRight. iPureIntro. lia.
-  Qed.
+  (*   iExists ss', s2. *)
+  (*   iSplitPure; first done. *)
+  (*   iSplit. *)
+  (*   { rewrite /crashed_in. *)
+  (*     iExists CV. *)
+  (*     iFrame "crashed crashedIn". *)
+  (*     iSplit; last (iPureIntro; apply elem_of_dom; done). *)
+  (*     iFrame. *)
+  (*     iExists (offset + tC), (offset + tC). *)
+  (*     assert ((offset + tC - (offset + tC)) = 0) as -> by lia. *)
+  (*     iFrame "persisted". *)
+  (*     iFrame "#∗". *)
+  (*     iDestruct (have_SV_0) as "$". *)
+  (*     iDestruct (have_FV_0) as "$". } *)
+  (*   iExists tLo, (offset + tC), (offset + tC), ∅, _, (Msg _ ∅ ∅ ∅), _. *)
+  (*   iFrame. iFrame "#". *)
+  (*   iSplitPure. { apply last_snoc. } *)
+  (*   iSplitPure. *)
+  (*   { apply: increasing_map_fmap. *)
+  (*     apply increasing_map_filter. *)
+  (*     done. } *)
+  (*   iSplitPure. *)
+  (*   { rewrite lookup_fmap. *)
+  (*     rewrite drop_above_lookup_t. *)
+  (*     rewrite absHistLook. *)
+  (*     done. } *)
+  (*   iSplitPure. { *)
+  (*     apply map_no_later_fmap. *)
+  (*     apply map_no_later_drop_above. } *)
+  (*   iSplitPure. *)
+  (*   { rewrite -fmap_snoc. *)
+  (*     apply map_sequence_fmap. *)
+  (*     apply map_sequence_drop_above. *)
+  (*     done. } *)
+  (*   iSplit. { simpl. iApply monPred_in_bottom. } *)
+  (*   iSplitPure; first lia. *)
+  (*   iSplitPure; first lia. *)
+  (*   iRight. iPureIntro. lia. *)
+  (* Qed. *)
 
-  Global Instance mapsto_na_into_crash ℓ `{!ProtocolConditions prot} q (ss : list ST) :
-    IntoCrash (ℓ ↦_{prot}^{q} ss)%I _ := post_crash_mapsto_na ℓ prot q ss.
+  (* TODO: restore this lemma *)
+  (* Global Instance mapsto_na_into_crash ℓ `{!ProtocolConditions prot} q (ss : list ST) : *)
+  (*   IntoCrash (ℓ ↦_{prot}^{q} ss)%I _ := post_crash_mapsto_na ℓ prot q ss. *)
 
-  (* This lemma is strictly weaker than the above but could be useful if we do
-  not want to preserve the prefix after a crash. *)
-  Lemma post_crash_mapsto_na_singleton ℓ `{!ProtocolConditions prot} q (ss : list ST) :
-    ℓ ↦_{prot}^{q} ss -∗
-    <PC> if_rec ℓ (∃ s,
-        ⌜ s ∈ ss ⌝ ∗
-        crashed_in prot ℓ s ∗
-        ℓ ↦_{prot}^{q} [prot.(p_bumper) s]).
-  Proof.
-    iIntros "pts".
-    iModIntro. iModIntro.
-    iDestruct "pts" as (???) "(crashed & pts)".
-    iExists s.
-    iSplitPure.
-    { eapply elem_of_list_lookup_2.
-      eapply prefix_lookup_Some; last done.
-      erewrite <- last_lookup.
-      apply last_snoc. }
-    iDestruct (crashed_in_persist_lb with "[$]") as "#per".
-  Abort. (* This should be true but is a bit annoying to show. *)
+  (* (* This lemma is strictly weaker than the above but could be useful if we do *)
+  (* not want to preserve the prefix after a crash. *) *)
+  (* Lemma post_crash_mapsto_na_singleton ℓ `{!ProtocolConditions prot} q (ss : list ST) : *)
+  (*   ℓ ↦_{prot}^{q} ss -∗ *)
+  (*   <PC> if_rec ℓ (∃ s, *)
+  (*       ⌜ s ∈ ss ⌝ ∗ *)
+  (*       crashed_in prot ℓ s ∗ *)
+  (*       ℓ ↦_{prot}^{q} [prot.(p_bumper) s]). *)
+  (* Proof. *)
+  (*   iIntros "pts". *)
+  (*   iModIntro. iModIntro. *)
+  (*   iDestruct "pts" as (???) "(crashed & pts)". *)
+  (*   iExists s. *)
+  (*   iSplitPure. *)
+  (*   { eapply elem_of_list_lookup_2. *)
+  (*     eapply prefix_lookup_Some; last done. *)
+  (*     erewrite <- last_lookup. *)
+  (*     apply last_snoc. } *)
+  (*   iDestruct (crashed_in_persist_lb with "[$]") as "#per". *)
+  (* Abort. (* This should be true but is a bit annoying to show. *) *)
 
-  Global Instance mapsto_na_into_crash_flush ℓ `{!ProtocolConditions prot} q
-      (ss : list ST) :
-    IntoCrashFlush _ _ :=
-    (into_crash_into_crash_flushed _ _ (post_crash_mapsto_na ℓ prot q ss)).
+  (* TODO: restore this lemma *)
+  (* Global Instance mapsto_na_into_crash_flush ℓ `{!ProtocolConditions prot} q *)
+  (*     (ss : list ST) : *)
+  (*   IntoCrashFlush _ _ := *)
+  (*   (into_crash_into_crash_flushed _ _ (post_crash_mapsto_na ℓ prot q ss)). *)
 
-  Lemma post_crash_flush_flush_lb (ℓ : loc) prot (s : ST) :
-    flush_lb ℓ prot s ⊢
-    <PCF> persist_lb ℓ prot (p_bumper prot s) ∗
-              ∃ s__pc, ⌜ s ⊑ s__pc ⌝ ∗ crashed_in prot ℓ s__pc.
-  Proof.
-    iNamed 1. iNamed "lbBase".
-    iNamed "locationProtocol".
-    iDestruct (post_crash_frag_history
-      with "knowPreorder offset knowBumper knowFragHist") as "HI".
-    iDestruct (post_crash_know_bumper with "knowBumper") as "bumper".
-    iDestruct (post_crash_preorder with "knowPreorder") as "order".
-    iCrashIntro.
-    iAssert (_)%I with "[viewFact]" as "pers".
-    { iDestruct "viewFact" as "[pers | pers]".
-      - iApply "pers".
-      - iDestruct "pers" as "($ & (%CV & % & % & ?))".
-        iExists _, _. iFrame. done. }
-    iDestruct "pers" as "(#persisted & (%CV & %t & (%cvLook & %le) & #crashed))".
-    iApply (if_rec_get with "crashed persisted"); first done.
-    iModIntro.
+  (* Lemma post_crash_flush_flush_lb (ℓ : loc) prot (s : ST) : *)
+  (*   flush_lb ℓ prot s ⊢ *)
+  (*   <PCF> persist_lb ℓ prot (p_bumper prot s) ∗ *)
+  (*             ∃ s__pc, ⌜ s ⊑ s__pc ⌝ ∗ crashed_in prot ℓ s__pc. *)
+  (* Proof. *)
+  (*   iNamed 1. iNamed "lbBase". *)
+  (*   iNamed "locationProtocol". *)
+  (*   iDestruct (post_crash_frag_history *)
+  (*     with "knowPreorder offset knowBumper knowFragHist") as "HI". *)
+  (*   iDestruct (post_crash_know_bumper with "knowBumper") as "bumper". *)
+  (*   iDestruct (post_crash_preorder with "knowPreorder") as "order". *)
+  (*   iCrashIntro. *)
+  (*   iAssert (_)%I with "[viewFact]" as "pers". *)
+  (*   { iDestruct "viewFact" as "[pers | pers]". *)
+  (*     - iApply "pers". *)
+  (*     - iDestruct "pers" as "($ & (%CV & % & % & ?))". *)
+  (*       iExists _, _. iFrame. done. } *)
+  (*   iDestruct "pers" as "(#persisted & (%CV & %t & (%cvLook & %le) & #crashed))". *)
+  (*   iApply (if_rec_get with "crashed persisted"); first done. *)
+  (*   iModIntro. *)
 
-    iDestruct "offset" as (???) "[crashed' offset]".
-    iDestruct (crashed_at_d_agree with "crashed crashed'") as %<-.
-    iClear "crashed'".
-    simplify_eq.
-    iDestruct "HI" as (?????) "(#crashed' & ? & #hist & ? & impl)".
-    iDestruct (crashed_at_d_agree with "crashed crashed'") as %<-.
-    iClear "crashed'".
-    simplify_eq.
-    iDestruct ("impl" with "[%]") as "[%incl ?]"; first lia.
-    iSplit.
-    - iExists _, _.
-      iFrame "∗#".
-      assert (tF - (offset + t) = 0) as -> by lia.
-      iDestruct (have_SV_0) as "$".
-      iDestruct (have_FV_0) as "$".
-      iFrame "persisted".
-    - iExists sC.
-      iFrame (incl).
-      iExists _. iFrame "∗#".
-      iSplit; last (iPureIntro; apply elem_of_dom; try naive_solver).
-      iExists _, _. iFrame "∗#".
-      replace (offset + t - (offset + t)) with 0 by lia.
-      iFrame "persisted".
-      iDestruct (have_SV_0) as "$".
-      iDestruct (have_FV_0) as "$".
-  Qed.
+  (*   iDestruct "offset" as (???) "[crashed' offset]". *)
+  (*   iDestruct (crashed_at_d_agree with "crashed crashed'") as %<-. *)
+  (*   iClear "crashed'". *)
+  (*   simplify_eq. *)
+  (*   iDestruct "HI" as (?????) "(#crashed' & ? & #hist & ? & impl)". *)
+  (*   iDestruct (crashed_at_d_agree with "crashed crashed'") as %<-. *)
+  (*   iClear "crashed'". *)
+  (*   simplify_eq. *)
+  (*   iDestruct ("impl" with "[%]") as "[%incl ?]"; first lia. *)
+  (*   iSplit. *)
+  (*   - iExists _, _. *)
+  (*     iFrame "∗#". *)
+  (*     assert (tF - (offset + t) = 0) as -> by lia. *)
+  (*     iDestruct (have_SV_0) as "$". *)
+  (*     iDestruct (have_FV_0) as "$". *)
+  (*     iFrame "persisted". *)
+  (*   - iExists sC. *)
+  (*     iFrame (incl). *)
+  (*     iExists _. iFrame "∗#". *)
+  (*     iSplit; last (iPureIntro; apply elem_of_dom; try naive_solver). *)
+  (*     iExists _, _. iFrame "∗#". *)
+  (*     replace (offset + t - (offset + t)) with 0 by lia. *)
+  (*     iFrame "persisted". *)
+  (*     iDestruct (have_SV_0) as "$". *)
+  (*     iDestruct (have_FV_0) as "$". *)
+  (* Qed. *)
 
-  Global Instance know_flush_into_crash ℓ prot (s : ST) :
-    IntoCrashFlush (flush_lb ℓ prot s) _ := post_crash_flush_flush_lb ℓ prot s.
-
-  Global Instance post_crash_into_crash P :
-    IntoCrash (post_crash P) P.
-  Proof. done. Qed.
+  (* TODO: restore this lemma *)
+  (* Global Instance know_flush_into_crash ℓ prot (s : ST) : *)
+  (*   IntoCrashFlush (flush_lb ℓ prot s) _ := post_crash_flush_flush_lb ℓ prot s. *)
 
   Lemma mapsto_at_store_lb ℓ prot ss s :
     ℓ ↦_AT^{prot} (ss ++ [s]) ⊢ store_lb ℓ prot s.
@@ -782,172 +776,173 @@ Section mapsto_at_lemmas.
     iNamed 1. iPureIntro. eapply increasing_map_to_increasing_list; done.
   Qed.
 
-  Lemma post_crash_mapsto_at_singleton ℓ prot (ss : list ST) :
-    ℓ ↦_AT^{prot} ss ⊢
-    <PC>
-      if_rec ℓ (∃ sC,
-        crashed_in prot ℓ sC ∗
-        ℓ ↦_AT^{prot} [prot.(p_bumper) sC]).
-  Proof.
-    rewrite /mapsto_at.
-    iNamed 1.
-    iDestruct (know_protocol_extract with "locationProtocol")
-      as "(pred & knowPreorder & knowBumper)".
-    iAssert (□ ∀ t s, know_frag_history_loc_d ℓ t s -∗ _)%I as "#impl".
-    { iIntros "!>" (??).
-      iApply (post_crash_frag_history with "knowPreorder offset knowBumper"). }
-    iDestruct (big_sepM_impl with "absHist []") as "HI".
-    { iIntros "!>" (???).
-      iApply "impl". }
-    iCrashIntro.
-    iDestruct (if_rec_is_persisted ℓ) as "persisted".
-    (* TODO: Why is this [IntoIfRec] instance not picked up automatically. *)
-    iDestruct (into_if_rec with "HI") as "HH".
-    { apply big_sepM_into_if_rec. intros. apply into_if_rec_if_rec. }
-    iModIntro.
-    iDestruct "offset" as (tC CV cvLook) "(crashed & #offset)".
-    iDestruct (big_sepM_lookup with "HH")
-      as (sC CV' tC' ? ?) "(#hi & #crashedIn & #frag & #phys & #hi2)".
-    { erewrite <- lastEq. eapply map_sequence_lookup_hi. done. }
-    iDestruct (crashed_at_d_agree with "crashed hi") as %<-.
-    assert (tC = tC') as <- by congruence.
-    (* Note, [sC] is the last location that was recovered after the crash.
-     * However, this location may not be among the locations in [ss]. *)
-    iExists (sC).
-    iSplitL "locationProtocol".
-    { iExists _. iFrame "hi crashedIn".
-      iSplit; last first.
-      - iPureIntro. apply elem_of_dom. done.
-      - rewrite /persist_lb.
-        iExists (offset + tC), (offset + tC).
-        replace (offset + tC - (offset + tC)) with 0 by lia.
-        iFrame "persisted".
-        iDestruct (have_FV_0) as "$".
-        rewrite /lb_base.
-        iFrameF "locationProtocol".
-        iFrameF "frag".
-        iFrameF "offset".
-        replace (offset + tC - (offset + tC)) with 0 by lia.
-        iDestruct (have_SV_0) as "$". }
+  (* TODO: restore this lemma *)
+  (* Lemma post_crash_mapsto_at_singleton ℓ prot (ss : list ST) : *)
+  (*   ℓ ↦_AT^{prot} ss ⊢ *)
+  (*   <PC> *)
+  (*     if_rec ℓ (∃ sC, *)
+  (*       crashed_in prot ℓ sC ∗ *)
+  (*       ℓ ↦_AT^{prot} [prot.(p_bumper) sC]). *)
+  (* Proof. *)
+  (*   rewrite /mapsto_at. *)
+  (*   iNamed 1. *)
+  (*   iDestruct (know_protocol_extract with "locationProtocol") *)
+  (*     as "(pred & knowPreorder & knowBumper)". *)
+  (*   iAssert (□ ∀ t s, know_frag_history_loc_d ℓ t s -∗ _)%I as "#impl". *)
+  (*   { iIntros "!>" (??). *)
+  (*     iApply (post_crash_frag_history with "knowPreorder offset knowBumper"). } *)
+  (*   iDestruct (big_sepM_impl with "absHist []") as "HI". *)
+  (*   { iIntros "!>" (???). *)
+  (*     iApply "impl". } *)
+  (*   iCrashIntro. *)
+  (*   iDestruct (if_rec_is_persisted ℓ) as "persisted". *)
+  (*   (* TODO: Why is this [IntoIfRec] instance not picked up automatically. *) *)
+  (*   iDestruct (into_if_rec with "HI") as "HH". *)
+  (*   { apply big_sepM_into_if_rec. intros. apply into_if_rec_if_rec. } *)
+  (*   iModIntro. *)
+  (*   iDestruct "offset" as (tC CV cvLook) "(crashed & #offset)". *)
+  (*   iDestruct (big_sepM_lookup with "HH") *)
+  (*     as (sC CV' tC' ? ?) "(#hi & #crashedIn & #frag & #phys & #hi2)". *)
+  (*   { erewrite <- lastEq. eapply map_sequence_lookup_hi. done. } *)
+  (*   iDestruct (crashed_at_d_agree with "crashed hi") as %<-. *)
+  (*   assert (tC = tC') as <- by congruence. *)
+  (*   (* Note, [sC] is the last location that was recovered after the crash. *)
+  (*    * However, this location may not be among the locations in [ss]. *) *)
+  (*   iExists (sC). *)
+  (*   iSplitL "locationProtocol". *)
+  (*   { iExists _. iFrame "hi crashedIn". *)
+  (*     iSplit; last first. *)
+  (*     - iPureIntro. apply elem_of_dom. done. *)
+  (*     - rewrite /persist_lb. *)
+  (*       iExists (offset + tC), (offset + tC). *)
+  (*       replace (offset + tC - (offset + tC)) with 0 by lia. *)
+  (*       iFrame "persisted". *)
+  (*       iDestruct (have_FV_0) as "$". *)
+  (*       rewrite /lb_base. *)
+  (*       iFrameF "locationProtocol". *)
+  (*       iFrameF "frag". *)
+  (*       iFrameF "offset". *)
+  (*       replace (offset + tC - (offset + tC)) with 0 by lia. *)
+  (*       iDestruct (have_SV_0) as "$". } *)
 
-    iExists ({[ (offset + tC) := _ ]}). iExistsN.
-    iSplitPure; first by reflexivity.
-    iFrame "#∗".
-    iSplitPure.
-    { split; first apply lookup_singleton. reflexivity. }
-    iSplitPure.
-    { apply map_sequence_singleton. }
-    iSplitPure.
-    { apply map_no_later_singleton. }
-    iSplitPure.
-    { rewrite 2!dom_singleton_L. done. }
-    iSplitPure; first apply increasing_map_singleton.
-    rewrite !big_sepM_singleton.
-    iFrameF "frag".
-    iSplit.
-    { iFrame "phys".
-      iApply have_msg_after_fence_empty. }
-    simpl.
-    replace (offset + tC - (offset + tC)) with 0 by lia.
-    iApply have_SV_0.
-  Qed.
+  (*   iExists ({[ (offset + tC) := _ ]}). iExistsN. *)
+  (*   iSplitPure; first by reflexivity. *)
+  (*   iFrame "#∗". *)
+  (*   iSplitPure. *)
+  (*   { split; first apply lookup_singleton. reflexivity. } *)
+  (*   iSplitPure. *)
+  (*   { apply map_sequence_singleton. } *)
+  (*   iSplitPure. *)
+  (*   { apply map_no_later_singleton. } *)
+  (*   iSplitPure. *)
+  (*   { rewrite 2!dom_singleton_L. done. } *)
+  (*   iSplitPure; first apply increasing_map_singleton. *)
+  (*   rewrite !big_sepM_singleton. *)
+  (*   iFrameF "frag". *)
+  (*   iSplit. *)
+  (*   { iFrame "phys". *)
+  (*     iApply have_msg_after_fence_empty. } *)
+  (*   simpl. *)
+  (*   replace (offset + tC - (offset + tC)) with 0 by lia. *)
+  (*   iApply have_SV_0. *)
+  (* Qed. *)
 
   (* NOTE: This lemma is (very likely) sound and is strictly stronger than the
    * lemma above. We have, however, not had a need for it yet and thus the
    * proof is aborted (for now). *)
-  Lemma post_crash_mapsto_at ℓ prot (ss : list ST) :
-    ℓ ↦_AT^{prot} ss ⊢
-    <PC> if_rec ℓ (∃ sC,
-        crashed_in prot ℓ sC ∗
-        (* At least one of our states are still there. *)
-        ((∃ ss1 s ss2,
-          ⌜ ss1 ++ [s] ++ ss2 = ss ⌝ ∗
-          ⌜ ∀ s2, head ss2 = Some s2 → sC ⊑ s2 ⌝ ∗
-          ⌜ s ⊑ sC ⌝ ∗
-          ℓ ↦_AT^{prot} ((prot.(p_bumper) <$> ss1) ++ [prot.(p_bumper) s])) ∨
-        (* None of our states where recovered. *)
-        ∃ sF,
-          ⌜ head ss = Some sF ∧ sC ⊑ sF ∧ sC ≠ sF ⌝ ∗
-          ℓ ↦_AT^{prot} [prot.(p_bumper) sC])
-      ).
-  Proof.
-    rewrite /mapsto_at.
-    iNamed 1.
-    iDestruct (know_protocol_extract with "locationProtocol")
-      as "(pred & order & bumper)".
-    iAssert (□ ∀ t s, know_frag_history_loc_d ℓ t s -∗ _)%I as "#impl".
-    { iIntros "!>" (??).
-      iApply (post_crash_frag_history with "order offset bumper"). }
-    iDestruct (big_sepM_impl with "absHist []") as "HI".
-    { iIntros "!>" (???).
-      iApply "impl". }
-    iCrashIntro.
-    iDestruct (if_rec_is_persisted ℓ) as "persisted".
-    (* TODO: Why is this [IntoIfRec] instance not picked up automatically. *)
-    iDestruct (into_if_rec with "HI") as "HH".
-    { apply big_sepM_into_if_rec. intros. apply into_if_rec_if_rec. }
-    iModIntro.
-    iDestruct "locationProtocol" as "#locationProtocol".
-    iDestruct "offset" as (tC CV cvLook) "(crashed & #offset)".
-    iDestruct (big_sepM_lookup with "HH")
-      as (sC CV' tC' ??) "(#hi & #crashedIn & #frag & ? & #hi2)".
-    { erewrite <- lastEq. eapply map_sequence_lookup_hi. done. }
-    iDestruct (crashed_at_d_agree with "crashed hi") as %<-.
-    assert (tC = tC') as <- by congruence.
-    (* Note, [sC] is the last location that was recovered after the crash.
-     * However, this location may not be among the locations in [ss]. *)
-    iExists (sC).
-    iSplitL "".
-    { iExists _. iFrame "hi crashedIn".
-      iSplit; last first.
-      - iPureIntro. apply elem_of_dom. done.
-      - rewrite /persist_lb.
-        iExists (offset + tC), (offset + tC).
-        replace (offset + tC - (offset + tC)) with 0 by lia.
-        iFrame "persisted".
-        iDestruct (have_FV_0) as "$".
-        iFrameF "locationProtocol".
-        iFrameF "frag".
-        iFrameF "offset".
-        replace (offset + tC - (offset + tC)) with 0 by lia.
-        iDestruct (have_SV_0) as "$". }
+  (* Lemma post_crash_mapsto_at ℓ prot (ss : list ST) : *)
+  (*   ℓ ↦_AT^{prot} ss ⊢ *)
+  (*   <PC> if_rec ℓ (∃ sC, *)
+  (*       crashed_in prot ℓ sC ∗ *)
+  (*       (* At least one of our states are still there. *) *)
+  (*       ((∃ ss1 s ss2, *)
+  (*         ⌜ ss1 ++ [s] ++ ss2 = ss ⌝ ∗ *)
+  (*         ⌜ ∀ s2, head ss2 = Some s2 → sC ⊑ s2 ⌝ ∗ *)
+  (*         ⌜ s ⊑ sC ⌝ ∗ *)
+  (*         ℓ ↦_AT^{prot} ((prot.(p_bumper) <$> ss1) ++ [prot.(p_bumper) s])) ∨ *)
+  (*       (* None of our states where recovered. *) *)
+  (*       ∃ sF, *)
+  (*         ⌜ head ss = Some sF ∧ sC ⊑ sF ∧ sC ≠ sF ⌝ ∗ *)
+  (*         ℓ ↦_AT^{prot} [prot.(p_bumper) sC]) *)
+  (*     ). *)
+  (* Proof. *)
+  (*   rewrite /mapsto_at. *)
+  (*   iNamed 1. *)
+  (*   iDestruct (know_protocol_extract with "locationProtocol") *)
+  (*     as "(pred & order & bumper)". *)
+  (*   iAssert (□ ∀ t s, know_frag_history_loc_d ℓ t s -∗ _)%I as "#impl". *)
+  (*   { iIntros "!>" (??). *)
+  (*     iApply (post_crash_frag_history with "order offset bumper"). } *)
+  (*   iDestruct (big_sepM_impl with "absHist []") as "HI". *)
+  (*   { iIntros "!>" (???). *)
+  (*     iApply "impl". } *)
+  (*   iCrashIntro. *)
+  (*   iDestruct (if_rec_is_persisted ℓ) as "persisted". *)
+  (*   (* TODO: Why is this [IntoIfRec] instance not picked up automatically. *) *)
+  (*   iDestruct (into_if_rec with "HI") as "HH". *)
+  (*   { apply big_sepM_into_if_rec. intros. apply into_if_rec_if_rec. } *)
+  (*   iModIntro. *)
+  (*   iDestruct "locationProtocol" as "#locationProtocol". *)
+  (*   iDestruct "offset" as (tC CV cvLook) "(crashed & #offset)". *)
+  (*   iDestruct (big_sepM_lookup with "HH") *)
+  (*     as (sC CV' tC' ??) "(#hi & #crashedIn & #frag & ? & #hi2)". *)
+  (*   { erewrite <- lastEq. eapply map_sequence_lookup_hi. done. } *)
+  (*   iDestruct (crashed_at_d_agree with "crashed hi") as %<-. *)
+  (*   assert (tC = tC') as <- by congruence. *)
+  (*   (* Note, [sC] is the last location that was recovered after the crash. *)
+  (*    * However, this location may not be among the locations in [ss]. *) *)
+  (*   iExists (sC). *)
+  (*   iSplitL "". *)
+  (*   { iExists _. iFrame "hi crashedIn". *)
+  (*     iSplit; last first. *)
+  (*     - iPureIntro. apply elem_of_dom. done. *)
+  (*     - rewrite /persist_lb. *)
+  (*       iExists (offset + tC), (offset + tC). *)
+  (*       replace (offset + tC - (offset + tC)) with 0 by lia. *)
+  (*       iFrame "persisted". *)
+  (*       iDestruct (have_FV_0) as "$". *)
+  (*       iFrameF "locationProtocol". *)
+  (*       iFrameF "frag". *)
+  (*       iFrameF "offset". *)
+  (*       replace (offset + tC - (offset + tC)) with 0 by lia. *)
+  (*       iDestruct (have_SV_0) as "$". } *)
 
-    (* Sketch: Case on wether tC+offset is below tLo or not. If it is above
-     * show left disjunct. Case on whether sC is equal to sF. If it is equal
-     * show left disjunct. If not show right disjunct. *)
-    destruct (decide (tLo ≤ tC + offset)).
-    (* - iLeft. *)
-    (* - *)
-  Abort.
+  (*   (* Sketch: Case on wether tC+offset is below tLo or not. If it is above *)
+  (*    * show left disjunct. Case on whether sC is equal to sF. If it is equal *)
+  (*    * show left disjunct. If not show right disjunct. *) *)
+  (*   destruct (decide (tLo ≤ tC + offset)). *)
+  (*   (* - iLeft. *) *)
+  (*   (* - *) *)
+  (* Abort. *)
 
-  Global Instance mapsto_at_into_crash ℓ prot ss : IntoCrash _ _ :=
-    post_crash_mapsto_at_singleton ℓ prot ss.
+  (* Global Instance mapsto_at_into_crash ℓ prot ss : IntoCrash _ _ := *)
+  (*   post_crash_mapsto_at_singleton ℓ prot ss. *)
 
-  Global Instance mapsto_at_into_crash_flush ℓ prot ss : IntoCrashFlush _ _ :=
-      into_crash_into_crash_flushed _ _ (post_crash_mapsto_at_singleton ℓ prot ss).
+  (* Global Instance mapsto_at_into_crash_flush ℓ prot ss : IntoCrashFlush _ _ := *)
+  (*     into_crash_into_crash_flushed _ _ (post_crash_mapsto_at_singleton ℓ prot ss). *)
 
-  Lemma post_crash_mapsto_na_flush_lb ℓ prot ss (s : ST) :
-    flush_lb ℓ prot s -∗
-    ℓ ↦_AT^{prot} (ss ++ [s]) -∗
-    <PCF>
-      persist_lb ℓ prot (prot.(p_bumper) s) ∗
-      ℓ ↦_AT^{prot} ((prot.(p_bumper) <$> ss) ++ [prot.(p_bumper) s]).
-  Proof.
-    (* iIntros "fLb pts". *)
-    (* iDestruct (mapsto_at_increasing with "pts") as %incr. *)
-    (* iModIntro. *)
-    (* iDestruct "fLb" as "[pLb (%sC & %le & #xCr)]". *)
-    (* iDestruct (crashed_in_if_rec with "xCr pts") as (?) "(xCr' & disj)". *)
-    (* iDestruct (crashed_in_agree with "xCr xCr'") as %<-. *)
-    (* iDestruct "disj" as "[H|H]"; last first. *)
-    (* { iDestruct "H" as (? ([= eq] & le2 & neq)) "H". *)
-    (*   rewrite head_lookup in eq. *)
-    (*   assert (s = sC). *)
-    (*   eapply increasing_list_last_greatest in incr; try done. *)
-    (*   2: { apply _. } *)
-    (*   2: { apply last_snoc. } *)
-    (*   (1* destruct sC; try done. *1) *)
-  Abort.
+  (* Lemma post_crash_mapsto_na_flush_lb ℓ prot ss (s : ST) : *)
+  (*   flush_lb ℓ prot s -∗ *)
+  (*   ℓ ↦_AT^{prot} (ss ++ [s]) -∗ *)
+  (*   <PCF> *)
+  (*     persist_lb ℓ prot (prot.(p_bumper) s) ∗ *)
+  (*     ℓ ↦_AT^{prot} ((prot.(p_bumper) <$> ss) ++ [prot.(p_bumper) s]). *)
+  (* Proof. *)
+  (*   (* iIntros "fLb pts". *) *)
+  (*   (* iDestruct (mapsto_at_increasing with "pts") as %incr. *) *)
+  (*   (* iModIntro. *) *)
+  (*   (* iDestruct "fLb" as "[pLb (%sC & %le & #xCr)]". *) *)
+  (*   (* iDestruct (crashed_in_if_rec with "xCr pts") as (?) "(xCr' & disj)". *) *)
+  (*   (* iDestruct (crashed_in_agree with "xCr xCr'") as %<-. *) *)
+  (*   (* iDestruct "disj" as "[H|H]"; last first. *) *)
+  (*   (* { iDestruct "H" as (? ([= eq] & le2 & neq)) "H". *) *)
+  (*   (*   rewrite head_lookup in eq. *) *)
+  (*   (*   assert (s = sC). *) *)
+  (*   (*   eapply increasing_list_last_greatest in incr; try done. *) *)
+  (*   (*   2: { apply _. } *) *)
+  (*   (*   2: { apply last_snoc. } *) *)
+  (*   (*   (1* destruct sC; try done. *1) *) *)
+  (* Abort. *)
 
 End mapsto_at_lemmas.
 
