src/high/modalities.v
@@ -1,24 +1,19 @@
-From iris.algebra Require Import gmap numbers.
 From iris.bi Require Import derived_laws.
 From iris.base_logic Require Import base_logic.
 From iris.proofmode Require Import base tactics classes.
 
-From Perennial.base_logic.lib Require Import ncfupd.
-
 From self.algebra Require Import view.
 From self.lang Require Import memory.
-From self.base Require Import primitive_laws.
-From self.high Require Import dprop dprop_liftings resources.
+From self.base Require Import primitive_laws generational_resources.
+From self.high Require Import dprop.
 
 Program Definition post_fence {Σ} (P : dProp Σ) : dProp Σ :=
-  MonPred (λ i, P ((store_view (i.1),
-                     (flush_view i.1 ⊔ buffer_view i.1),
-                     buffer_view i.1), i.2)) _.
+  MonPred (λ TV, P (store_view TV,
+                    (flush_view TV ⊔ buffer_view TV),
+                    buffer_view TV)) _.
   (* MonPred (λ '(s, p, b), P (s, (p ⊔ b), ∅)) _. *)
 Next Obligation.
-  intros Σ P.
-  do 2 intros [[[??]?]?].
-  intros [[[??]?] [= ->]].
+  intros Σ P. intros [[??]?] [[??]?] [[??]?]. simpl.
   assert (g0 ⊔ g1 ⊑ g3 ⊔ g4). { solve_proper. }
   apply monPred_mono.
   rewrite !subseteq_prod'.
@@ -28,21 +23,17 @@ Qed.
 Notation "'<fence>' P" :=
   (post_fence P) (at level 20, right associativity) : bi_scope.
 
-Program Definition post_fence_sync `{nvmBaseFixedG Σ}
+Program Definition post_fence_sync `{!nvmBaseG Σ Ω}
         (P : dProp Σ) : dProp Σ :=
-  MonPred (λ i,
-    let nD := i.2 in
+  MonPred (λ TV,
     bi_wand
-      (persisted (buffer_view i.1))
-      (P ((store_view i.1,
-          (flush_view i.1 ⊔ buffer_view i.1),
-           buffer_view i.1), i.2))
+      (persisted (buffer_view TV))
+      (P (store_view TV,
+          (flush_view TV ⊔ buffer_view TV),
+           buffer_view TV))
   ) _.
 Next Obligation.
-  intros Σ ??.
-  do 2 intros [[[??]?]?].
-  intros [[[??]?] [= ->]].
-  simpl.
+  intros Σ ?? P. intros [[??]?] [[??]?] [[??]?]. simpl.
   assert (g0 ⊔ g1 ⊑ g3 ⊔ g4). { solve_proper. }
   iIntros "pers P".
   iApply monPred_mono; last iApply "pers".
@@ -55,11 +46,9 @@ Notation "'<fence_sync>' P" :=
   (post_fence_sync P) (at level 20, right associativity) : bi_scope.
 
 Program Definition no_buffer `{Σ : gFunctors} (P : dProp Σ) : dProp Σ :=
-  MonPred (λ i, P (store_view i.1, flush_view i.1, ∅, i.2)) _.
+  MonPred (λ TV, P (store_view TV, flush_view TV, ∅)) _.
 Next Obligation.
-  intros Σ P.
-  do 2 intros [[[??]?]?]. intros [[[??]?] [= ->]].
-  simpl.
+  intros Σ P. intros [[??]?] [[??]?] [[??]?]. simpl.
   apply monPred_mono.
   rewrite !subseteq_prod'.
   done.
@@ -69,10 +58,9 @@ Notation "'<nobuf>' P" :=
   (no_buffer P) (at level 20, right associativity) : bi_scope.
 
 Program Definition no_flush `{Σ : gFunctors} (P : dProp Σ) : dProp Σ :=
-  MonPred (λ i, P (store_view i.1, ∅, ∅, i.2)) _.
+  MonPred (λ TV, P (store_view TV, ∅, ∅)) _.
 Next Obligation.
-  intros Σ P.
-  do 2 intros [[[??]?]?]. intros [[[??]?] [= ->]].
+  intros Σ P. intros [[??]?] [[??]?] [[??]?]. simpl.
   apply monPred_mono.
   rewrite !subseteq_prod'.
   done.
