src/high/protocol.v
@@ -1,17 +1,18 @@
-From iris.base_logic.lib Require Import own.
-From iris.proofmode Require Import reduction monpred tactics.
+From iris.proofmode Require Import proofmode.
 From iris_named_props Require Import named_props.
 
+From self.high.lib Require Import abstract_state.
 From self Require Import encode_relation.
-From self.high Require Import dprop dprop_liftings resources modalities
-  post_crash_modality monpred_simpl or_lost if_rec predicates.
+
+From self.high Require Import dprop generational_resources modalities monpred_simpl predicates wrappers.
+From self.high.modalities Require Import no_buffer nextgen if_rec.
+
 From self.lang Require Import lang.
-From self.high.modalities Require Import no_buffer.
 
 (* A handy alias for the type of location predicates. *)
-Definition loc_pred `{nvmG Σ} ST `{AbstractState ST} := ST → val → dProp Σ.
+Definition loc_pred `{nvmHighG} ST `{AbstractState ST} := ST → val → dProp Σ.
 
-Definition loc_predO `{nvmG Σ} ST := ST -d> val -d> dPropO Σ.
+Definition loc_predO `{nvmHighG} ST := ST -d> val -d> dPropO Σ.
 
 
 (* A protocol consists of
@@ -19,41 +20,41 @@ Definition loc_predO `{nvmG Σ} ST := ST -d> val -d> dPropO Σ.
     location.
   - A function [bumper] that specifies how the state of a location changes
     after a crash. *)
-Record LocationProtocol ST `{AbstractState ST, nvmG Σ} := MkProt {
+Record LocationProtocol ST `{AbstractState ST, nvmHighG} := MkProt {
   p_inv : loc_pred ST;
   p_bumper : ST → ST;
 }.
 
-Global Arguments MkProt {_} {_} {_} {_} {_} {_} _%I _%I.
+Global Arguments MkProt   {_ _ _ _ _ _ _ _} _%I _.
 
-Global Arguments p_inv {ST} {_} {_} {_} {_} {_} _.
-Global Arguments p_bumper {ST} {_} {_} {_} {_} {_} _.
+Global Arguments p_inv    {ST _ _ _ _ _ _ _} _.
+Global Arguments p_bumper {ST _ _ _ _ _ _ _} _ _.
 
 (* Type class collection the properties that a protocol should have.
 
 Note: The fields are ordered by "difficulty" in the sense of how difficult these
 conditions usually are to show.  *)
-Class ProtocolConditions `{AbstractState ST, nvmG Σ} (prot : LocationProtocol ST) := {
+Class ProtocolConditions `{AbstractState ST, nvmHighG} (prot : LocationProtocol ST) := {
   bumper_mono :
     Proper ((⊑@{ST}) ==> (⊑))%signature (prot.(p_bumper));
   inv_nobuf :>
     ∀ s v, BufferFree (prot.(p_inv) s v);
   pred_condition :
-    (⊢ ∀ s v, prot.(p_inv) s v -∗ <PCF> prot.(p_inv) (prot.(p_bumper) s) v : dProp Σ)%I;
+    (⊢ ∀ s v, prot.(p_inv) s v -∗ nextgen (prot.(p_inv) (prot.(p_bumper) s) v) : dProp Σ)%I;
 }.
 
-#[global] Hint Mode ProtocolConditions + + + + + + ! : typeclass_instances.
+#[global] Hint Mode ProtocolConditions + + + + + + + + ! : typeclass_instances.
 
 Existing Instance bumper_mono.
 Existing Instance inv_nobuf.
 
 (** [know_protocol] represents the knowledge that a location is associated with a
 specific protocol. It's defined simply using more "primitive" assertions. *)
-Definition know_protocol `{AbstractState ST, nvmG Σ}
+Definition know_protocol `{AbstractState ST, nvmHighG}
            ℓ (prot : LocationProtocol ST) : dProp Σ :=
-  "#knowPred" ∷ know_pred_d ℓ prot.(p_inv) ∗
-  "#knowPreorder" ∷ know_preorder_loc_d ℓ (⊑@{ST}) ∗
-  "#knowBumper" ∷ know_bumper ℓ prot.(p_bumper).
+  "#knowPred" ∷ ⎡ know_pred ℓ prot.(p_inv) ⎤ ∗
+  "#knowPreorder" ∷ ⎡ know_preorder_loc ℓ (⊑@{ST}) ⎤ ∗
+  "#knowBumper" ∷ ⎡ know_bumper ℓ prot.(p_bumper) ⎤.
 
 Lemma encode_bumper_bump_mono `{AbstractState ST}
       (bumper : ST → ST) `{!Proper ((⊑@{ST}) ==> (⊑))%signature bumper}
@@ -71,48 +72,51 @@ Proof.
 Qed.
 
 Section protocol.
-  Context `{nvmG Σ, AbstractState ST}.
+  Context `{nvmHighG, AbstractState ST}.
 
   Implicit Types (prot : LocationProtocol ST).
 
-  Lemma post_crash_know_protocol ℓ prot :
-    know_protocol ℓ prot -∗ <PC> if_rec ℓ (know_protocol ℓ prot).
+  Lemma nextgen_know_protocol ℓ prot :
+    know_protocol ℓ prot -∗ nextgen $ if_rec ℓ (know_protocol ℓ prot).
   Proof.
-    iIntros "(a & b & c)".
-    iModIntro. iModIntro. iFrame.
+    iNamed 1.
+    iModIntro.
+    iDestruct "knowBumper" as "[% ?]".
+    rewrite -?if_rec_lift_if_rec.
+    iModIntro. iFrame "#%".
   Qed.
 
-  Global Instance know_protocol_into_crash ℓ prot :
-    IntoCrash
+  Global Instance know_protocol_into_nextgen ℓ prot :
+    IntoNextgen
       (know_protocol ℓ prot)
       (if_rec ℓ (know_protocol ℓ prot)).
   Proof.
-    rewrite /IntoCrash. iIntros "P". by iApply post_crash_know_protocol.
+    rewrite /IntoNextgen. iIntros "P". by iApply nextgen_know_protocol.
   Qed.
 
   Lemma know_protocol_extract ℓ prot :
     know_protocol ℓ prot -∗
-      know_pred_d ℓ prot.(p_inv) ∗
-      know_preorder_loc_d ℓ (⊑@{ST}) ∗
-      know_bumper ℓ prot.(p_bumper).
+      ⎡ know_pred ℓ prot.(p_inv) ⎤ ∗
+      ⎡ know_preorder_loc ℓ (⊑@{ST}) ⎤ ∗
+      ⎡ know_bumper ℓ prot.(p_bumper) ⎤.
   Proof. iNamed 1. iFrame "#". Qed.
 
   Lemma know_protocol_unfold ℓ prot i :
     know_protocol ℓ prot i ⊣⊢
-       ("#knowPred" ∷ know_pred_d ℓ (p_inv prot) i ∗
-        "#knowPreorder" ∷ know_preorder_loc_d ℓ (⊑@{ST}) i ∗
-        "#knowBumper" ∷ know_bumper ℓ (p_bumper prot) i).
-  Proof. rewrite /know_protocol !monPred_at_sep //. Qed.
+    ("#knowPred" ∷ know_pred ℓ (p_inv prot) ∗
+     "#knowPreorder" ∷ know_preorder_loc ℓ (⊑@{ST}) ∗
+     "#knowBumper" ∷ know_bumper ℓ (p_bumper prot)).
+  Proof. rewrite /know_protocol !monPred_at_sep !monPred_at_embed //. Qed.
 
   Global Instance know_protocol_buffer_free ℓ prot :
     BufferFree (know_protocol ℓ prot).
   Proof. apply _. Qed.
 
-  Lemma know_protocol_at ℓ prot TV gnames :
-    (know_protocol ℓ prot) (TV, gnames) ⊣⊢
-      know_pred ℓ prot.(p_inv) ∗
-      know_preorder_loc ℓ (⊑@{ST}) ∗
-      own_know_bumper (get_bumpers_name gnames) ℓ prot.(p_bumper).
+  Lemma know_protocol_at ℓ prot TV :
+    (know_protocol ℓ prot) TV ⊣⊢
+    know_pred ℓ prot.(p_inv) ∗
+    know_preorder_loc ℓ (⊑@{ST}) ∗
+    know_bumper ℓ prot.(p_bumper).
   Proof.
     rewrite /know_protocol. rewrite !monPred_at_sep.
     simpl. rewrite !monPred_at_embed.
@@ -123,16 +127,11 @@ Section protocol.
     Contractive (λ (inv : loc_predO ST), (know_protocol ℓ (MkProt inv bumper))).
   Proof.
     rewrite /know_protocol.
-    rewrite /know_pred_d.
     intros ????.
     f_equiv; last done.
     f_equiv.
     f_equiv.
-    intros ?? ->.
     f_contractive.
     assumption.
   Qed.
-
 End protocol.
-
-Opaque know_protocol.
