src/high/resources/gen_predicates.v
@@ -11,18 +11,20 @@ From self Require Import extra map_extra.
 From self.nextgen Require Import hvec nextgen_promises.
 From self.algebra Require Import view.
 From self.base Require Import generational_resources.
+From self.base.modalities Require Import if_rec.
 
 From self.lang Require Import lang.
 
 Definition predicateR Σ :=
   agreeR (positive -d> val -d> laterO (optionO (thread_view -d> iPropO Σ))).
-Definition predicatesR Σ := gmap_viewR loc (predicateR Σ).
+Definition predicatesR Σ := authR (gmapUR loc (predicateR Σ)).
 Notation predicates_inG Σ Ω := (genInDepsG Σ Ω (predicatesR Σ) [#crashed_atR]).
 
 Section ownership.
   Context `{!nvmBaseG Σ Ω, !predicates_inG Σ Ω}.
   Implicit Type (OCV: view) (PRs: gmap loc (predicateR Σ)) (PR: predicateR Σ).
 
+  (* TODO: both this definition and the lemma below are duplicates *)
   Definition drop_OCV OCV ℓ PR :=
     if (decide (ℓ ∈ dom OCV)) then Some PR else None.
 
@@ -32,21 +34,94 @@ Section ownership.
     λ tC t,
       ∃ OCV,
         tC = crashed_at_trans OCV ∧
-        t = map_entry_lift_gmap_view $ drop_OCV OCV.
+        t = fmap_auth $ map_imap $ drop_OCV OCV.
 
   Definition own_all_preds_ra γ dq PRs: iProp Σ :=
-    ∃ OCV,
-      "own_auth" ∷ gen_own γ (gmap_view_auth dq PRs) ∗
-      "#crashed" ∷ crashed_at_offset OCV ∗
-      "#rely" ∷ rely γ [#crashed_at_name] predicates_rel True_pred.
+    "own_auth" ∷ gen_own γ (●{dq} PRs) ∗
+    "#rely" ∷ rely γ [#crashed_at_name] predicates_rel True_pred ∗
+    "#crashed" ∷ ∃ OCV, crashed_at_offset OCV.
 
-  Definition know_pred_ra γ ℓ dq PR: iProp Σ :=
-    ∃ OCV,
-      "own_frag" ∷ gen_own γ (gmap_view_frag ℓ dq PR) ∗
-      "#crashed" ∷ crashed_at_offset OCV ∗
-      "#rely" ∷ rely γ [#crashed_at_name] predicates_rel True_pred.
+  Definition know_pred_ra γ ℓ PR: iProp Σ :=
+    "own_frag" ∷ gen_own γ (◯ {[ ℓ := PR ]}) ∗
+    "#rely" ∷ rely γ [#crashed_at_name] predicates_rel True_pred ∗
+    "#crashed" ∷ ∃ OCV, crashed_at_offset OCV.
 
-  (* TODO: put relevant lemmas here *)
+  Lemma map_imap_drop_OCV_restrict OCV m:
+    map_imap (drop_OCV OCV) m = restrict (dom OCV) m.
+  Proof.
+    apply map_eq => i.
+    rewrite /drop_OCV map_lookup_imap /=.
+    destruct (decide (i ∈ dom OCV)).
+    - rewrite restrict_lookup_elem_of; last done.
+      by destruct (m !! i).
+    - rewrite restrict_lookup_not_elem_of; last done.
+      by destruct (m !! i).
+  Qed.
+
+  Global Instance own_all_preds_auth_into_nextgen γ dq PRs:
+    IntoNextgen
+      (own_all_preds_ra γ dq PRs)
+      (∃ OCV,
+          own_all_preds_ra γ dq (restrict (dom OCV) PRs) ∗
+          picked_in crashed_at_name (crashed_at_trans OCV)).
+  Proof.
+    rewrite /IntoNextgen.
+    iNamed 1.
+    iDestruct "crashed" as (OCV) "crashed".
+    iModIntro.
+    iDestruct ("own_auth") as (t) "[#picked own_auth]".
+    iDestruct "rely" as "(rely & (%t' & %tC & (%R & _) & picked' & pickedC))".
+    iPickedInAgree "picked picked'".
+    destruct R as (OCV' & -> & ->).
+    iExists OCV'.
+    rewrite fmap_auth_auth.
+    iDestruct "own_auth" as "[own_auth _]".
+    iDestruct "crashed" as (??) "[pickedC' #crashed_at]".
+    iPickedInAgree "pickedC pickedC'".
+    iEval (simpl) in "crashed_at".
+    rewrite map_imap_drop_OCV_restrict.
+    iFrame "∗#".
+    iExists _, _.
+    iApply "crashed_at".
+  Qed.
+
+  Global Instance ghost_map_elem_into_nextgen γ k PR:
+    IntoNextgen
+      (know_pred_ra γ k PR)
+      (if_rec k (know_pred_ra γ k PR)).
+  Proof.
+    rewrite /IntoNextgen.
+    iNamed 1.
+    iDestruct "crashed" as (OCV) "crashed".
+    iModIntro.
+    iDestruct "own_frag" as (t) "[#picked frag]".
+    iDestruct "rely" as "(rely & (%t' & %tC & (%R & _) & picked' & pickedC))".
+    iPickedInAgree "picked picked'".
+    destruct R as (OCV' & -> & ->).
+    iIntros (CV [[t] ?]) "#crashed_at #persisted_loc".
+    iAssert ⌜ k ∈ dom OCV' ⌝%I as "%".
+    { iDestruct "crashed_at" as (??? Hview) "[crashed_at _]".
+      iDestruct "crashed" as (??) "[pickedC' #crashed_at']".
+      iPickedInAgree "pickedC pickedC'".
+      iDestruct (gen_own_valid_2 with "crashed_at' crashed_at") as %[_ <-%to_agree_op_valid_L]%pair_valid.
+      iPureIntro.
+      rewrite -(view_sub_dom_eq _ OV) Hview.
+      rewrite elem_of_dom.
+      by eexists.
+    }
+    rewrite fmap_auth_frag.
+    (* TODO: move to separate lemma *)
+    rewrite -{1}insert_empty.
+    erewrite map_imap_insert_Some;
+      first rewrite map_imap_empty insert_empty //;
+        last rewrite /drop_OCV decide_True //.
+    iDestruct "crashed" as (??) "[pickedC' #crashed_at']".
+    iPickedInAgree "pickedC pickedC'".
+    iFrame "∗#".
+    iIntros.
+    iExists _, _.
+    iApply "crashed_at'".
+  Qed.
 End ownership.
 
 Arguments predicateR {Σ}.
