src/high/modalities/nextgen.v
@@ -1,0 +1,269 @@
+(** This file defines the lifted [nextgen] modality for [monPred] *)
+From iris.proofmode Require Import proofmode.
+
+From self.high.lib Require Import abstract_state.
+
+From self.base Require Import generational_resources.
+From self.high Require Import dprop.
+From self.nextgen Require Export nextgen_promises.
+
+Definition nextgen `{nvmBaseG} (P: dProp Σ): dProp Σ := MonPred (λ TV, ⚡==> P (∅, ∅, ∅))%I _.
+
+Class IntoNextgen `{nvmBaseG} (P Q : dProp Σ) :=
+  into_nextgen : P ⊢ nextgen Q.
+Global Arguments IntoNextgen {_ _ _} _%I _%I.
+Global Arguments into_nextgen {_ _ _} _%I _%I.
+Global Hint Mode IntoNextgen + + + + - : typeclass_instances.
+
+Section Modality.
+  Context `{nvmBaseG}.
+
+  Set Default Proof Using "Type*".
+
+  Implicit Types (P Q: dProp Σ).
+
+  Lemma nextgen_mono (P Q: dProp Σ) :
+    (P ⊢ Q) → nextgen P ⊢ nextgen Q.
+  Proof.
+    intros Hi.
+    iStartProof (iProp _); iIntros (?).
+    simpl.
+    iApply nextgen_mono.
+    iApply Hi.
+  Qed.
+
+  Global Instance nextgen_mono' :
+    Proper ((⊢) ==> (⊢)) (nextgen).
+  Proof. intros P Q. apply nextgen_mono. Qed.
+
+  (* Global Instance nextgen_ne : NonExpansive nextgen. *)
+  (* Proof.  solve_proper. Qed. *)
+
+  (* Global Instance nextgen_proper : Proper ((≡) ==> (≡)) nextgen := ne_proper _. *)
+
+  Lemma nextgen_intuitionistic P Q:
+    IntoNextgen P Q → □ P ⊢ nextgen (□ Q).
+  Proof.
+    intros Hi.
+    iStartProof (iProp _); iIntros (?).
+    rewrite Hi.
+    simpl.
+    rewrite monPred_at_intuitionistically.
+    rewrite 2!bi.intuitionistically_into_persistently.
+    iApply nextgen_intuitionistically_2.
+  Qed.
+
+  Lemma nextgen_and P Q:
+    nextgen P ∧ nextgen Q ⊢ nextgen (P ∧ Q).
+  Proof.
+    intros.
+    iStartProof (iProp _); iIntros (?). simpl.
+    rewrite monPred_at_and.
+    rewrite nextgen_and_1.
+    naive_solver.
+  Qed.
+
+  Lemma nextgen_emp:
+    emp ⊢ nextgen emp.
+  Proof.
+    iStartProof (iProp _); iIntros (?). simpl.
+    rewrite monPred_at_emp.
+    iApply nextgen_emp_2.
+  Qed.
+
+  Lemma nextgen_sep P Q:
+    nextgen P ∗ nextgen Q ⊢ nextgen (P ∗ Q).
+  Proof.
+    iStartProof (iProp _). iIntros (TV).
+    simpl.
+    rewrite monPred_at_sep.
+    iApply nextgen_sep_2.
+  Qed.
+
+  Lemma modality_nextgen_mixin :
+    modality_mixin (@nextgen _ _ _)
+      (MIEnvTransform IntoNextgen) (MIEnvTransform IntoNextgen).
+  Proof.
+    split; simpl; split_and?.
+    - apply nextgen_intuitionistic.
+    - apply nextgen_and.
+    - done.
+    - apply nextgen_emp.
+    - apply nextgen_mono.
+    - apply nextgen_sep.
+  Qed.
+  Definition modality_nextgen :=
+    Modality _ modality_nextgen_mixin.
+
+  Global Instance from_modal_nextgen (P: dProp Σ) :
+    FromModal True modality_nextgen (nextgen P) (nextgen P) P | 1.
+  Proof. by rewrite /FromModal. Qed.
+
+  Global Instance into_nextgen_into_nextgen (P Q: iProp Σ) :
+    nextgen_promises_model.IntoNextgen P Q → IntoNextgen ⎡ P ⎤ ⎡ Q ⎤.
+  Proof.
+    rewrite /IntoNextgen /IntoNextgen.
+    intros Hi.
+    iStartProof (iProp _); iIntros (?). simpl.
+    rewrite Hi.
+    rewrite monPred_at_embed.
+    naive_solver.
+  Qed.
+End Modality.
+
+Notation "'<NG>' P" := (nextgen P)
+  (at level 200, right associativity) : bi_scope.
+
+Section IntoNextgen.
+  Context `{nvmBaseG}.
+
+  (* Arguments IntoNextgen {_} {_} {_} _%I hi%I. *)
+
+  Global Instance sep_into_crash (P Q : dProp Σ) (P' Q' : dProp Σ) :
+    IntoNextgen P P' →
+    IntoNextgen Q Q' →
+    IntoNextgen (P ∗ Q)%I (P' ∗ Q')%I.
+  Proof.
+    rewrite /IntoNextgen.
+    iIntros (Pi Qi) "[P Q]".
+    iDestruct (Pi with "P") as "P".
+    iDestruct (Qi with "Q") as "Q".
+    iApply (nextgen_sep). iFrame.
+  Qed.
+
+  Global Instance pure_into_crash (P : Prop) :
+    IntoNextgen (⌜ P ⌝) (⌜ P ⌝)%I.
+  Proof. rewrite /IntoNextgen. iIntros "%". by iModIntro. Qed.
+
+  Lemma into_crash_proper P P' Q Q':
+    IntoNextgen P Q →
+    (P ⊣⊢ P') →
+    (Q ⊣⊢ Q') →
+    IntoNextgen P' Q'.
+  Proof.
+    rewrite /IntoNextgen.
+    iIntros (HD Hwand1 Hwand2) "HP".
+    iApply nextgen_mono; last first.
+    { iApply HD. iApply Hwand1. eauto. }
+    intros. simpl. by rewrite Hwand2.
+  Qed.
+
+  Global Instance big_sepM_into_crash `{Countable K} :
+    ∀ (A : Type) Φ (Ψ : K → A → dProp Σ) (m : gmap K A),
+    (∀ (k : K) (x : A), IntoNextgen (Φ k x) (Ψ k x)) →
+    IntoNextgen ([∗ map] k↦x ∈ m, Φ k x)%I ([∗ map] k↦x ∈ m, Ψ k x)%I.
+  Proof.
+    intros. induction m using map_ind.
+    - eapply (into_crash_proper True%I _ True%I).
+      * apply _.
+      * rewrite big_sepM_empty. apply bi.True_emp.
+      * intros. rewrite big_sepM_empty. apply bi.True_emp.
+    - eapply (into_crash_proper (Φ i x ∗ [∗ map] k↦x0 ∈ m, Φ k x0) _
+                                ((Ψ i x ∗ [∗ map] k↦x0 ∈ m, Ψ k x0)%I)).
+      * apply _.
+      * rewrite big_sepM_insert //=.
+      * intros. rewrite big_sepM_insert //=.
+  Qed.
+
+  Tactic Notation "lift_into_nextgen" uconstr(lem) :=
+    rewrite /IntoNextgen; iIntros "P"; by iApply lem.
+
+  Global Instance emp_into_crash : IntoNextgen emp emp.
+  Proof. lift_into_nextgen nextgen_emp. Qed.
+
+  (* TODO: verify this is indeed impossible *)
+  (* Global Instance disj_into_crash (P Q : dProp Σ) (P' Q' : dProp Σ) : *)
+  (*   IntoNextgen P P' → IntoNextgen Q Q' → IntoNextgen (P ∨ Q)%I (P' ∨ Q')%I. *)
+  (* Proof. *)
+  (*   rewrite /IntoNextgen. *)
+  (*   iIntros (Pi Qi) "[P|Q]". *)
+  (*   - iDestruct (Pi with "P") as "P". *)
+  (*     iApply nextgen_disj. *)
+  (*     iLeft. *)
+  (*     iFrame. *)
+  (*   - iDestruct (Qi with "Q") as "Q". *)
+  (*     iApply post_crash_disj. *)
+  (*     iRight. *)
+  (*     iFrame. *)
+  (* Qed. *)
+
+  (* Global Instance later_into_crash_flush P P' : *)
+  (*   IntoNextgen P P' → *)
+  (*   IntoNextgen (▷ P) (▷ P'). *)
+  (* Proof. *)
+  (*   intros (?). *)
+  (*   rewrite /IntoNextgen. *)
+  (*   iModel. *)
+  (*   iIntros "H". *)
+  (* Qed. *)
+
+  Global Instance exist_into_crash {A} Φ Ψ:
+    (∀ x : A, IntoNextgen (Φ x) (Ψ x)) →
+    IntoNextgen (∃ x, Φ x)%I ((∃ x, Ψ x)%I).
+  Proof.
+    rewrite /IntoNextgen.
+    iIntros (Hc) "H". iDestruct "H" as (?) "HΦ". iPoseProof (Hc with "[$]") as "HΦ".
+    iApply (nextgen_mono with "HΦ"). auto.
+  Qed.
+
+  (* Global Instance embed_into_crash P : *)
+  (*   IntoNextgen (⎡ P ⎤%I) (λ _, ⎡ P ⎤%I). *)
+  (* Proof. rewrite /IntoNextgen. iIntros "P". by iApply post_crash_embed_nodep. Qed. *)
+End IntoNextgen.
+
+Section nextgen_derived.
+  Context `{nvmBaseG} `{AbstractState ST}.
+
+  (* TODO: if this lemma is required, prove it in base logic. *)
+  (* Lemma post_crash_persisted_loc_d ℓ t : *)
+  (*   persisted_loc_d ℓ t ⊢ *)
+  (*   <PC> ( *)
+  (*     persisted_loc_d ℓ 0 ∗ *)
+  (*     ∃ CV t', ⌜ CV !! ℓ = Some (MaxNat t') ∧ t ≤ t' ⌝ ∗ crashed_at_d CV)%I. *)
+  (* Proof. *)
+  (*   iIntros "P". *)
+  (*   iDestruct (post_crash_persisted_d with "P") as "P". *)
+  (*   iApply (post_crash_mono with "P"). *)
+  (*   rewrite view_to_zero_singleton. *)
+  (*   iIntros "[$ M]". *)
+  (*   setoid_rewrite view_le_singleton. *)
+  (*   setoid_rewrite bi.pure_exist. *)
+  (*   setoid_rewrite bi.sep_exist_r. *)
+  (*   done. *)
+  (* Qed. *)
+
+  (* Global Instance into_crash_persisted_loc_d ℓ t : *)
+  (*   IntoNextgen _ _ := post_crash_persisted_loc_d ℓ t. *)
+
+  (* Lemma post_crash_know_frag_history_loc ℓ t (s : ST) : *)
+  (*   ⎡ know_preorder_loc ℓ (⊑@{ST}) ∗ *)
+  (*     know_frag_history_loc ℓ {[ t := s ]} ∗ *)
+  (*     persisted {[ ℓ := MaxNat t]} ⎤ -∗ *)
+  (*   post_crash (λ nD', *)
+  (*     ∃ s' t' CV, *)
+  (*       ⌜ s ⊑ s' ⌝ ∗ *)
+  (*       ⌜ t ≤ t' ⌝ ∗ *)
+  (*       ⌜ CV !! ℓ = Some (MaxNat t') ⌝ ∗ *)
+  (*       ⎡ know_preorder_loc (nD := nD') ℓ (abs_state_relation (ST := ST)) ∗ *)
+  (*         know_frag_history_loc ℓ {[ 0 := s' ]} ∗ *)
+  (*         crashed_at CV ∗ *)
+  (*         persisted {[ ℓ := MaxNat 0 ]} ⎤ *)
+  (*   ). *)
+  (* Proof. *)
+  (*   iStartProof (dProp _). *)
+  (*   iIntros "(order & hist & pers)". *)
+  (*   iCrash. *)
+  (*   iDestruct "pers" as "[pers (%CV & %t' & [%cvLook %le] & #crash)]". *)
+  (*   iDestruct (or_lost_get with "[$] order") as "order"; first naive_solver. *)
+  (*   iDestruct "hist" as (CV') "[crash' [hist | %cvLook']]"; *)
+  (*     iDestruct (crashed_at_agree with "crash crash'") as %<-; last congruence. *)
+  (*   iClear "crash'". *)
+  (*   iDestruct "hist" as (? cvLook' s' impl) "fragHist". *)
+  (*   simplify_eq. *)
+  (*   iExists s', t', CV. *)
+  (*   iFrame. *)
+  (*   iFrame "#". *)
+  (*   naive_solver. *)
+  (* Qed. *)
+
+End nextgen_derived.
