src/high/modalities/nextgen_flush.v
@@ -1,0 +1,351 @@
+From iris.proofmode Require Import proofmode.
+From iris_named_props Require Import named_props.
+
+From iris.bi Require Import monpred.
+From self.nextgen Require Export nextgen_promises.
+From self.base Require Import generational_resources primitive_laws.
+From self.high Require Import dprop monpred_simpl.
+From self.high.modalities Require Import nextgen.
+
+From self.algebra Require Import view.
+
+Program Definition nextgen_flush `{nvmBaseG} (P : dProp Σ) : dProp Σ :=
+  MonPred (λ TV,
+    (<NG>
+      ∀ (CV : view),
+        ⌜ flush_view TV ⊑ CV ⌝ ∗
+        ⎡ persisted (view_to_zero (flush_view TV)) ⎤ ∗
+        ⎡ crashed_at CV ⎤ -∗
+        P) (∅, ∅, ∅))%I _.
+Next Obligation.
+  intros ???????.
+  apply nextgen_mono.
+  solve_proper.
+Qed.
+
+Class IntoNGFlush `{nvmBaseG}
+      (P : dProp Σ) (Q : dProp Σ) :=
+  into_nextgen_flushed : P ⊢ nextgen_flush (Σ := Σ) Q.
+
+Arguments IntoNGFlush {_ _ _} _%I _%I.
+
+Notation "'<NGF>' P" :=
+  (nextgen_flush P)
+  (at level 200, right associativity) : bi_scope.
+
+Section nextgen_persisted.
+  Context `{nvmBaseG}.
+
+  Lemma nextgen_flush_nextgen P :
+    nextgen P ⊢ nextgen_flush P.
+  Proof.
+    iStartProof (iProp _).
+    iIntros (TV) "P".
+    rewrite /nextgen_flush.
+    rewrite /nextgen.
+    simpl.
+    iModIntro.
+    iIntros (CV TV') "% not_lost".
+    iApply monPred_mono; done.
+  Qed.
+
+  Lemma nextgen_flush_named P name :
+    named name (nextgen_flush P) ⊢
+    nextgen_flush (named name P).
+  Proof. rewrite //=. Qed.
+
+  Lemma nextgen_flush_sep P Q :
+    nextgen_flush P ∗ nextgen_flush Q ⊢ <NGF> P ∗ Q.
+  Proof.
+    iModel.
+    iIntros "(HP & HQ)".
+    rewrite /nextgen_flush //=.
+    iModIntro.
+    iIntros (CV TV') "% #not_lost".
+    iDestruct ("HP" $! CV with "[$]") as "HP".
+    iDestruct ("HQ" $! CV with "[$]") as "HQ".
+    iSplitL "HP"; iApply monPred_mono; done.
+  Qed.
+
+  Lemma nextgen_flush_disj P Q :
+    nextgen_flush P ∨ nextgen_flush Q -∗ <NGF> P ∨ Q.
+  Proof.
+    iModel.
+    rewrite /nextgen_flush //=.
+    iIntros "[HP | HQ]"; iModIntro; iIntros (CV TV') "% #not_lost".
+    - iDestruct ("HP" $! CV with "[$]") as "HP".
+      iLeft.
+      iApply monPred_mono; done.
+    - iDestruct ("HQ" $! CV with "[$]") as "HQ".
+      iRight.
+      iApply monPred_mono; done.
+  Qed.
+
+  Lemma nextgen_flush_mono P Q :
+    (P ⊢ Q) → nextgen_flush P ⊢ nextgen_flush Q.
+  Proof.
+    intros mono.
+    iModel.
+    rewrite /nextgen_flush //=.
+    iApply nextgen_promises_model.nextgen_mono.
+    iIntros "HP" (CV TV') "% #not_lost".
+    iDestruct ("HP" $! CV with "[$]") as "HP".
+    iApply mono.
+    iApply monPred_mono; done.
+  Qed.
+
+  Global Instance nextgen_flush_proper :
+    Proper ((⊣⊢) ==> (⊣⊢)) (nextgen_flush).
+  Proof.
+    intros ?? eq.
+    apply (anti_symm _).
+    - apply nextgen_flush_mono. rewrite eq. done.
+    - apply nextgen_flush_mono. rewrite eq. done.
+  Qed.
+
+  Lemma nextgen_flush_emp : emp ⊢ nextgen_flush emp.
+  Proof.
+    rewrite -nextgen_flush_nextgen. by iIntros "_ !>".
+  Qed.
+
+  Lemma modality_nextgen_flush_mixin :
+    modality_mixin (@nextgen_flush Σ _ _)
+      (MIEnvClear) (MIEnvTransform IntoNGFlush).
+  Proof.
+    split; simpl; split_and?;
+    eauto using bi.equiv_entails_1_2, nextgen_flush_emp,
+      nextgen_flush_mono, nextgen_flush_sep.
+
+    (* intros P Q. rewrite /IntoNextgen. => ->. *)
+    (* by rewrite nextgen_flush_intuitionistically_2. *)
+  Qed.
+  Definition modality_nextgen_flush :=
+    Modality _ modality_nextgen_flush_mixin.
+
+  Global Instance from_modal_nextgen_flush P :
+    FromModal True (modality_nextgen_flush) (<NGF> P) (<NGF> P) P.
+  Proof. by rewrite /FromModal. Qed.
+
+  Lemma nextgen_flush_pure (P : Prop) : P → ⊢ <NGF> ⌜P⌝.
+    rewrite -nextgen_flush_nextgen. by iIntros (?) "!>".
+  Qed.
+
+  Lemma nextgen_have_FV_strong ℓ t :
+    have_FV_strong ℓ t ⊢
+    <NGF>
+      ⎡ persisted {[ ℓ := MaxNat 0 ]} ⎤ ∗
+      ∃ CV t', ⌜CV !! ℓ = Some (MaxNat t') ∧ t ≤ t'⌝ ∗ ⎡ crashed_at CV ⎤.
+  Proof.
+    iModel. iIntros "le". simpl.
+    iModIntro.
+    iIntros (CV TV') "% (% & #? & #?)".
+    destruct (TV) as [[??]?].
+    iDestruct "le" as %[[? le] ?].
+    iDestruct (persisted_persisted_loc with "[$]") as "$".
+    { apply view_le_singleton in le as (t2 & look & ?).
+      eapply view_to_zero_lookup. done. }
+    iExists CV. iFrame "#".
+    iPureIntro.
+    apply view_le_singleton.
+    etrans; done.
+  Qed.
+End nextgen_persisted.
+
+Section IntoNGFlush.
+  Context `{nvmBaseG}.
+
+  (* This is not an instance as it would probably have a negative impact on the
+  performance of type class resolution. *)
+  (* TODO (Yixuan): verify performance *)
+  Global Instance into_crash_into_crash_flushed P Q :
+    IntoNextgen P Q →
+    IntoNGFlush P Q.
+  Proof.
+    rewrite /IntoNGFlush /IntoNextgen.
+    rewrite -nextgen_flush_nextgen.
+    done.
+  Qed.
+
+  (* Global Instance pure_into_crash_flushed (P : Prop) : *)
+  (*   IntoNGFlush (⌜ P ⌝) (⌜ P ⌝)%I. *)
+  (* Proof. apply into_crash_into_crash_flushed. apply _. Qed. *)
+
+  (* Global Instance lifted_embed_nodep_into_crash_flush (P : iProp Σ) : *)
+  (*   IntoNGFlush (⎡ P ⎤) (⎡ P ⎤)%I | 1000. *)
+  (* Proof. apply into_crash_into_crash_flushed. apply into_nextgen_into_nextgen. Qed. *)
+
+  (* Global Instance lifted_embed_into_crash_flush (P : iProp Σ) Q : *)
+  (*   base.nextgen_modality.IntoNextgen P Q → *)
+  (*   IntoNGFlush (⎡ P ⎤) (⎡ Q ⎤)%I. *)
+  (* Proof. intros ?. apply into_crash_into_crash_flushed. apply _. Qed. *)
+
+  (* Global Instance emp_into_crash_flush : IntoNGFlush emp emp. *)
+  (* Proof. apply _. apply: into_crash_into_crash_flushed. Qed. *)
+
+  Global Instance sep_into_crash_flush (P Q : dProp Σ) (P' Q' : dProp Σ) :
+    IntoNGFlush P P' →
+    IntoNGFlush Q Q' →
+    IntoNGFlush (P ∗ Q)%I (P' ∗ Q')%I.
+  Proof.
+    rewrite /IntoNGFlush.
+    iIntros (Pi Qi) "[P Q]".
+    iDestruct (Pi with "P") as "P".
+    iDestruct (Qi with "Q") as "Q".
+    iApply nextgen_flush_sep.
+    iFrame.
+  Qed.
+
+  Global Instance disj_into_crash_flush (P Q : dProp Σ) (P' Q' : dProp Σ) :
+    IntoNGFlush P P' →
+    IntoNGFlush Q Q' →
+    IntoNGFlush (P ∨ Q)%I (P' ∨ Q')%I.
+  Proof.
+    rewrite /IntoNGFlush.
+    iIntros (Pi Qi) "[P|Q]".
+    - iDestruct (Pi with "P") as "P".
+      iApply nextgen_flush_disj.
+      iLeft.
+      iFrame.
+    - iDestruct (Qi with "Q") as "Q".
+      iApply nextgen_flush_disj.
+      iRight.
+      iFrame.
+  Qed.
+
+  Global Instance if_else_into_crash_flush (b : bool) P P' Q Q' :
+    IntoNGFlush P P' →
+    IntoNGFlush Q Q' →
+    IntoNGFlush (if b then P else Q) (if b then P' else Q').
+  Proof. intros ??. destruct b; apply _. Qed.
+
+  (* Global Instance later_into_crash_flush P P' : *)
+  (*   IntoNGFlush P P' → *)
+  (*   IntoNGFlush (▷ P) (▷ P'). *)
+  (* Proof. *)
+  (* Qed. *)
+
+  Global Instance have_FV_strong_into_crash_flush ℓ t :
+    IntoNGFlush _ _ := nextgen_have_FV_strong ℓ t.
+
+  Global Instance exist_into_crash_flush {A} Φ Ψ:
+    (∀ x : A, IntoNGFlush (Φ x) (Ψ x)) →
+    IntoNGFlush (∃ x, Φ x) (∃ x, Ψ x).
+  Proof.
+    rewrite /IntoNGFlush.
+    iIntros (Hc) "H". iDestruct "H" as (?) "HΦ". iPoseProof (Hc with "[$]") as "HΦ".
+    iApply (nextgen_flush_mono with "HΦ"). auto.
+  Qed.
+
+  Global Instance big_sepL_into_crash_flush {A} ϕ ψ l :
+    (∀ k (x : A), IntoNGFlush (ϕ k x) (ψ k x)) →
+    IntoNGFlush ([∗ list] k↦x ∈ l, ϕ k x)%I ([∗ list] k↦x ∈ l, ψ k x)%I.
+  Proof. revert ϕ ψ. induction l as [|x l IH]=> Φ ψ ? /=; apply _. Qed.
+End IntoNGFlush.
+
+
+(* since I no longer import the other high level definitions, this test section is commentted. *)
+(* Section nextgen_flush_test. *)
+(*   From self.high Require Import predicates. *)
+(*   From self.high.modalities Require Import if_rec. *)
+(*   Context `{generational_resources.nvmHighG}. *)
+
+(*   Lemma foo P `{Countable ST'} ℓ (ϕ : ST' → val → dProp Σ) t : *)
+(*     ⌜ P ⌝ -∗ *)
+(*     ⎡ know_pred ℓ ϕ ⎤ -∗ *)
+(*     ⎡ persisted_loc ℓ t ⎤ -∗ *)
+(*     <NGF> ⌜ P ⌝ ∗ if_rec ℓ (⎡ know_pred ℓ ϕ ⎤). *)
+(*   Proof. *)
+(*     iIntros "P pred pers". *)
+(*     iModIntro. *)
+(*     rewrite if_rec_lift_if_rec. *)
+(*     iFrame. *)
+(*   Qed. *)
+
+(* End nextgen_flush_test. *)
+
+Typeclasses Opaque nextgen.
+Typeclasses Opaque nextgen_flush.
+
+(* Since the post crash modality does not satisfy
+   [nextgen_intuitionistically_2] the [iModIntro] tactic clears the
+   intuitionistic context when introducing the post crash modality. This is quite
+   unfortunate. To improve the situation we define [iCrashIntro] which improves on
+   this by moving the entire intuitionistic context into the spatial context before
+   introducing the post crash modality.
+
+   The tactic works both with <PC> and with <PCF>.
+ *)
+
+From iris.bi Require Import bi.
+Import bi.
+From iris.proofmode Require Import tactics environments intro_patterns monpred.
+
+Section intuit_to_spatial.
+  Context {PROP : bi}.
+
+  Implicit Types Γ Γp Γs : env PROP.
+  Implicit Types Δ : envs PROP.
+  Implicit Types P Q : PROP.
+
+  (* Lemma envs_clear_spatial_sound Δ : *)
+  (*   of_envs Δ ⊢ of_envs (envs_clear_spatial Δ) ∗ [∗] env_spatial Δ. *)
+  (* Proof. *)
+  (*   rewrite !of_envs_eq /envs_clear_spatial /=. apply pure_elim_l=> Hwf. *)
+  (*   rewrite -persistent_and_sep_assoc. apply and_intro. *)
+  (*   - apply pure_intro. destruct Hwf; constructor; simpl; auto using Enil_wf. *)
+  (*   - rewrite -persistent_and_sep_assoc. rewrite left_id. done. *)
+  (* Qed. *)
+
+  Lemma envs_clear_intuitionistic_sound Δ :
+    of_envs Δ ⊢
+    env_and_persistently (env_intuitionistic Δ) ∗ of_envs (envs_clear_intuitionistic Δ).
+  Proof.
+    rewrite !of_envs_eq /envs_clear_spatial /=. apply pure_elim_l=> Hwf.
+    rewrite persistent_and_sep_1.
+    rewrite (pure_True); first by rewrite !left_id.
+    destruct Hwf. constructor; simpl; auto using Enil_wf.
+  Qed.
+
+  Lemma big_opL_and_sep (l : env PROP) : □ [∧] l -∗ [∗] l.
+  Proof.
+    iInduction (l) as [|??] "IH"; simpl; first done.
+    iIntros "#[$ ?]". iApply "IH". done.
+  Qed.
+
+  Lemma big_opL_env_and_sep `{BiAffine PROP} (l : env PROP) :
+    env_and_persistently l ⊢ [∗] l.
+  Proof.
+    iInduction (l) as [|??] "IH"; simpl; first done.
+    iIntros "[#$ ?]". iApply "IH". done.
+  Qed.
+
+  Definition envs_intuitionistic_to_spatial {PROP} (Δ : envs PROP) : option (envs PROP) :=
+    envs_app false (env_intuitionistic Δ) (envs_clear_intuitionistic Δ).
+
+  Lemma envs_intuitionistic_to_spatial_sound `{BiAffine PROP} Δ Δ' P :
+    envs_intuitionistic_to_spatial Δ = Some Δ' →
+    envs_entails Δ' P →
+    envs_entails Δ P.
+  Proof.
+    rewrite /envs_intuitionistic_to_spatial.
+    intros eq.
+    rewrite envs_entails_unseal.
+    intros <-.
+    apply envs_app_sound in eq.
+    apply wand_elim_l' in eq.
+    rewrite <- eq.
+    rewrite envs_clear_intuitionistic_sound.
+    iIntros "[? $]".
+    rewrite -big_opL_env_and_sep.
+    done.
+  Qed.
+
+End intuit_to_spatial.
+
+(* Moves the intuitionistic context to the spatial context. *)
+Tactic Notation "iIntuitToSpatial" :=
+  eapply envs_intuitionistic_to_spatial_sound;
+    [ done
+    | cbv [ env_spatial ]].
+
+Tactic Notation "iCrashIntro" := iIntuitToSpatial; iModIntro.
