src/high/wrappers.v
@@ -1,0 +1,299 @@
+(** This file contains several wrapper definitions and their lemmas
+ ** base logic to high logic.
+
+ ** In spirea 1.0, wrappers were defined so that one can swap out the
+ ** ghost names easily. Even though that is no longer necessary, I'm redefining
+ ** them in similar shapes for minimal proof changes.
+
+ ** A key difference between spirea 1.0 and spirea 2.0 wrappers is that I decide to use
+ ** [⎡ P ⎤] whenever possible. This wasn't possible because generational ghost names were
+ ** part of the [BiIndex]. *)
+From iris.proofmode Require Import proofmode.
+From iris_named_props Require Import named_props.
+
+From iris.algebra Require Import gset.
+From self Require Import extra encode_relation.
+From self.high.lib Require Import abstract_state.
+
+From iris.bi.lib Require Import fractional.
+From self.nextgen Require Import nextgen_promises.
+From self.high Require Import generational_resources.
+
+(* For some reason [iris.algebra.view.view] always triumph the in-house definition. *)
+From self.algebra Require Export view.
+
+Set Default Proof Using "Type*".
+
+Section BaseLifting.
+  Context `{nvmBaseG}.
+
+  Definition offset_loc ℓ (t : nat) : iProp Σ :=
+    ∃ OCV, crashed_at_offset OCV ∗ ⌜ OCV !! ℓ = Some $ MaxNat t ⌝.
+
+  Lemma offset_loc_agree ℓ t1 t2 :
+    offset_loc ℓ t1 -∗
+    offset_loc ℓ t2 -∗
+    ⌜ t1 = t2 ⌝.
+  Proof.
+    rewrite /offset_loc.
+    iIntros "(% & ? & %) (% & ? & %)".
+    iDestruct (crashed_at_offset_agree with "[$] [$]") as "%".
+    by simplify_map_eq.
+  Qed.
+
+  Lemma offset_loc_crashed_at_agree ℓ t OCV :
+    offset_loc ℓ t -∗
+    crashed_at_offset (MaxNat <$> OCV) -∗
+    ⌜ OCV !! ℓ = Some $ t ⌝.
+  Proof.
+    iIntros "(%OCV' & offset1 & %look) offset2".
+    iDestruct (crashed_at_offset_agree with "offset1 offset2") as "->".
+    rewrite lookup_fmap in look.
+    destruct (OCV !! ℓ) eqn:Heqn; simpl in look; by simplify_eq.
+  Qed.
+
+  (* (* although the offset never decreases and thus a stronger lemma should be correct, *)
+  (*  * the way [crashed_at_trans] is defined right now doesn't guarantee that. *) *)
+  (* Global Instance offset_loc_into_nextgen ℓ t: *)
+  (*   IntoNextgen *)
+  (*   (offset_loc ℓ t) *)
+  (*   (∃ t', offset_loc ℓ t'). *)
+  (* Proof. *)
+  (*   rewrite /IntoNextgen. *)
+  (*   iIntros "offset !>". *)
+  (*   iDestruct "offset" as (OCV) "[(%OV & %trans & picked & offset) %]". *)
+
+End BaseLifting.
+
+Section location_sets.
+  Context `{nvmHighG}.
+  Implicit Types (locs : gset loc) (ℓ : loc).
+
+  Definition is_at_loc ℓ : iProp Σ :=
+    gen_alocs_frag shared_locs_name {[ ℓ ]}.
+  Definition is_na_loc ℓ : iProp Σ :=
+    gen_alocs_frag exclusive_locs_name {[ ℓ ]}.
+
+  Lemma location_sets_singleton_included {γ} locs ℓ :
+    gen_alocs_auth γ locs -∗ gen_alocs_frag γ {[ ℓ ]} -∗ ⌜ ℓ ∈ locs ⌝.
+  Proof.
+    iNamed 1. iNamed 1.
+    iDestruct (gen_own_valid_2 with "own_auth own_frag")
+      as %[V%gset_included _]%auth_both_valid_discrete.
+    rewrite elem_of_subseteq_singleton.
+    done.
+  Qed.
+
+  Lemma location_sets_lookup γ locs ℓ :
+    ℓ ∈ locs → gen_alocs_frag γ locs -∗ gen_alocs_frag γ {[ ℓ ]}.
+  Proof.
+    intros.
+    iNamed 1.
+    iPoseProof (gen_own_mono _ _ (◯ {[ ℓ ]}) with "own_frag") as "own_frag".
+    { apply auth_frag_mono. set_solver. }
+    iExists OCV.
+    iFrame "∗#".
+  Qed.
+End location_sets.
+
+Section preorders.
+  Context `{nvmHighG}.
+
+  Implicit Type (preorders : gmap loc (relation2 positive)).
+  Context `{Countable ST}.
+
+  Definition own_all_preorders γ preorders :=
+    ghost_map_auth γ loc_map_rel (DfracOwn 1) preorders.
+
+  Definition own_know_preorder_loc γ ℓ (preorder : relation2 ST) : iProp Σ :=
+    ℓ ↪[γ, loc_map_rel]□ encode_relation preorder.
+
+  Definition know_preorder_loc ℓ (preorder : relation2 ST) : iProp Σ :=
+    own_know_preorder_loc preorders_name ℓ preorder.
+
+  Lemma own_all_preorders_gname_alloc (preorders : gmap loc (relation2 positive)) :
+    ⊢ |==> ∃ γ,
+      own_all_preorders γ preorders ∗ ([∗ map] ℓ ↦ p ∈ preorders, ℓ ↪[γ, loc_map_rel]□ p).
+  Proof.
+  Admitted.
+
+  Lemma orders_lookup γ ℓ order1 order2 (orders : gmap loc (relation2 positive)) :
+    orders !! ℓ = Some order1 →
+    own_all_preorders γ orders -∗
+    own_know_preorder_loc γ ℓ order2 -∗
+    ⌜order1 = encode_relation order2⌝.
+  Proof.
+    iIntros (look) "auth frag".
+    iDestruct (ghost_map_lookup with "auth frag") as "%".
+    iPureIntro. congruence.
+  Qed.
+End preorders.
+
+(* Pure facts about bumpers *)
+Section bumpers.
+  Context `{AbstractState ST}.
+
+  Definition encode_bumper (bumper : ST → ST) :=
+    λ e, encode <$> (bumper <$> decode e).
+
+  Lemma encode_bumper_Some_decode (bumper : ST → ST) (x x' : positive) :
+    encode_bumper bumper x = Some x' →
+    ∃ (s : ST), decode x = Some s ∧ encode (bumper s) = x'.
+  Proof.
+    rewrite /encode_bumper => eq.
+    destruct (decode x) as [s|].
+    - exists s. inversion eq. done.
+    - inversion eq.
+  Qed.
+
+  Lemma encode_bumper_encode (bumper : ST → ST) (s : ST) :
+    encode_bumper bumper (encode s) = Some (encode (bumper s)).
+  Proof. rewrite /encode_bumper. rewrite decode_encode. done. Qed.
+
+  (* An encoded bumper returns some encoded value then that encoded value will
+  also result in some other encoded bumper again. This represents that encoded
+  bumpers take "valid" encodings to "valid" encodings. *)
+  Lemma encode_bumper_bump_to_valid bumper e e' :
+    encode_bumper bumper e = Some e' → is_Some (encode_bumper bumper e').
+  Proof.
+    intros (s' & ? & encodeEq)%encode_bumper_Some_decode.
+    rewrite <- encodeEq. rewrite encode_bumper_encode. done.
+  Qed.
+End bumpers.
+
+Section own_encoded_bumpers.
+  Context `{nvmHighG}.
+
+  Definition own_all_bumpers γ (encoded_bumpers: gmap loc (positive → option positive)) :=
+    ghost_map_auth γ loc_map_rel (DfracOwn 1) encoded_bumpers.
+
+  (* TODO: *)
+  Lemma own_all_bumpers_alloc bumpers :
+    ⊢ |==> ∃ γ, own_all_bumpers γ bumpers ∗
+                ([∗ map] ℓ ↦ bumper ∈ bumpers, ℓ ↪[γ, loc_map_rel]□ bumper).
+  Proof. Admitted.
+
+End own_encoded_bumpers.
+
+Section own_bumpers.
+  Context `{nvmHighG}.
+  Context `{AbstractState ST}.
+
+  Definition own_know_bumper γ (ℓ : loc) (bumper : ST → ST) : iProp Σ :=
+    let encodedBumper := encode_bumper bumper
+    in ⌜∀ s1 s2, s1 ⊑ s2 → bumper s1 ⊑ bumper s2⌝ ∗
+       ℓ ↪[γ, loc_map_rel]□ encodedBumper.
+
+  Definition know_bumper ℓ (bumper : ST → ST) : iProp Σ :=
+    own_know_bumper bumpers_name ℓ bumper.
+
+  Lemma own_all_bumpers_persist γ encoded_bumpers :
+    own_all_bumpers γ encoded_bumpers ==∗
+    ghost_map_auth γ loc_map_rel DfracDiscarded encoded_bumpers.
+  Proof. apply ghost_map_auth_persist. Qed.
+
+  Lemma own_all_bumpers_insert (bumpers : gmap loc _) ℓ γ (bumper : ST → ST)
+        `{!Proper ((⊑@{ST}) ==> (⊑))%signature bumper} :
+    bumpers !! ℓ = None →
+    own_all_bumpers γ bumpers ==∗
+    own_all_bumpers γ (<[ℓ := encode_bumper bumper]>bumpers) ∗ own_know_bumper γ ℓ bumper.
+  Proof.
+    rewrite /own_all_bumpers /own_know_bumper. iIntros (look) "A".
+    iMod (ghost_map_insert_persist with "A") as "[$ $]"; done.
+  Qed.
+
+  Definition bumperO := leibnizO (positive → option positive).
+
+  Lemma bumpers_lookup γ ℓ encoded_bumpers bumper :
+    own_all_bumpers γ encoded_bumpers -∗
+    own_know_bumper γ ℓ bumper -∗
+    ⌜ encoded_bumpers !! ℓ = Some (encode_bumper bumper) ⌝.
+  Proof.
+    iIntros "A [mono F]".
+    iDestruct (ghost_map_lookup with "A F") as "$".
+  Qed.
+End own_bumpers.
+
+Section NAView.
+  Context `{nvmHighG}.
+
+  Definition know_na_view ℓ q (SV : view) : iProp Σ :=
+    ℓ ↪[non_atomic_views_gname, loc_map_rel]{#q} SV%I.
+
+  Lemma know_na_view_agree ℓ p q V V' :
+    know_na_view ℓ q V -∗
+    know_na_view ℓ p V' -∗
+    ⌜ V = V' ⌝.
+  Proof.
+    iApply (ghost_map_elem_agree _ _ _ _ _ V).
+  Qed.
+
+  Global Instance know_na_view_fractional ℓ V :
+    Fractional (λ q, know_na_view ℓ q V).
+  Proof. apply _. Qed.
+
+  Global Instance know_na_view_as_fractional ℓ V q :
+    AsFractional (know_na_view ℓ q V)
+      (λ q, know_na_view ℓ q V) q.
+  Proof. apply _. Qed.
+End NAView.
+
+(* so that iDestruct will prioritize fractional lemma over splitting [gen_own] *)
+Global Opaque know_na_view.
+
+Section crashed_in.
+  Context `{nvmHighG}.
+  Context `{Countable ST}.
+
+  Definition crashed_in ℓ (s : ST) : iProp Σ :=
+    ∃ es, ⌜ decode es = Some s ⌝ ∗ ℓ ↪[crashed_in_name, loc_map_rel]□ es.
+End crashed_in.
+
+Section Histories.
+  Context `{nvmHighG}.
+
+  Definition know_full_encoded_history_loc ℓ q enc_abs_hist : iProp Σ :=
+    history_full_entry_encoded bumpers_name abs_history_name ℓ q enc_abs_hist.
+
+  Definition know_frag_encoded_history_loc ℓ t e : iProp Σ :=
+    frag_entry bumpers_name abs_history_name ℓ t e.
+
+  Definition know_phys_hist_msg ℓ t msg : iProp Σ :=
+    auth_map_map_frag_singleton phy_history_name ℓ t msg.
+
+  Context `{Countable ST}.
+
+  Definition know_full_history_loc `{Countable ST}
+             ℓ q (abs_hist : gmap time ST) : iProp Σ :=
+    full_entry_unenc bumpers_name abs_history_name ℓ q abs_hist.
+
+  Definition know_frag_history_loc `{Countable ST} ℓ t (s : ST) : iProp Σ :=
+    frag_entry_unenc bumpers_name abs_history_name ℓ t s.
+
+  Lemma know_full_entry_frag_entry_unenc ℓ q abs_hist t s :
+    know_full_history_loc ℓ q abs_hist -∗
+    know_frag_history_loc ℓ t s -∗
+    ⌜ abs_hist !! t = Some s ⌝.
+  Proof.
+    rewrite /know_full_history_loc.
+    rewrite /know_frag_history_loc.
+    iApply full_entry_frag_entry_unenc.
+  Qed.
+
+  Lemma know_full_history_loc_agree ℓ p q (abs_hist1 abs_hist2 : gmap nat ST) :
+    know_full_history_loc ℓ p abs_hist1 -∗
+    know_full_history_loc ℓ q abs_hist2 -∗
+    ⌜ abs_hist1 = abs_hist2 ⌝.
+  Proof.
+    iApply full_entry_unenc_agree.
+  Qed.
+
+  Global Instance know_full_history_loc_fractional ℓ (abs_hist : gmap nat ST) :
+    Fractional (λ q, know_full_history_loc ℓ q abs_hist).
+  Proof. apply _. Qed.
+
+  Global Instance know_full_history_loc_as_fractional ℓ (abs_hist : gmap nat ST) q :
+    AsFractional (know_full_history_loc ℓ q abs_hist)
+      (λ q, know_full_history_loc ℓ q abs_hist) q.
+  Proof. apply _. Qed.
+End Histories.
